wip on udp

theories/aneris_lang/state_interp.v
@@ -6,7 +6,18 @@ From iris_string_ident Require Import ltac2_string_ident.
 From aneris.program_logic Require Export weakestpre adequacy.
 From aneris.program_logic Require Import ectx_lifting.
 From aneris.program_logic Require Export gen_heap_light.
-From aneris.aneris_lang Require Export aneris_lang notation network resources.
+From aneris.aneris_lang Require Export
+     aneris_lang notation network resources
+     state_interp_def
+     state_interp_local_coh
+     state_interp_gnames_coh
+     state_interp_free_ips_coh
+     state_interp_network_sockets_coh
+     state_interp_socket_interp_coh
+     state_interp_messages_resource_coh
+     state_interp_messages_history_coh
+     state_interp_config_wp.
+
 From aneris.aneris_lang.lib Require Import util.
 
 From RecordUpdate Require Import RecordSet.
@@ -16,1369 +27,8 @@ Import uPred.
 Import Network.
 Import RecordSetNotations.
 
-Local Hint Extern 0 (head_reducible _ _) => eexists _, _, _; simpl : core.
-Local Hint Constructors head_step : core.
-Local Hint Resolve alloc_fresh : core.
-Local Hint Resolve to_of_val : core.
-
-(* TODO: come up with something more reliable *)
-Ltac ddeq k1 k2 :=
-  destruct (decide (k1 = k2)); subst;
-  repeat
-    match goal with
-    | Hyp : context[ (<[_:=_]>_) !! _ ] |- _ =>
-      rewrite lookup_insert in
-          Hyp || (rewrite lookup_insert_ne in Hyp; last done);
-      simplify_eq /=
-    | Hyp : is_Some _ |- _ => destruct Hyp
-    | |- context[ (<[_:=_]>_) !! _ ] =>
-      rewrite lookup_insert || (rewrite lookup_insert_ne; last done);
-      simplify_eq /=
-    |  H1 : ?x = ?z, Heq : ?x = ?y |- _ =>
-       rewrite Heq in H1; simplify_eq /=; try eauto
-    | Hdel : context[ delete ?n ?m !! ?n = _] |- _ =>
-      rewrite lookup_delete in Hdel; simplify_eq /=
-    end.
-
-Section definitions.
-  Context `{anerisG Σ}.
-  Implicit Types σ : state.
-  Implicit Types h : heap.
-  Implicit Types H : gmap ip_address heap.
-  Implicit Types S : gmap ip_address sockets.
-  Implicit Types Sn : sockets.
-  Implicit Types P : ports_in_use.
-  Implicit Types ps : gset port.
-  Implicit Types ips : gset ip_address.
-  Implicit Types M R T : message_soup.
-  Implicit Types m : message.
-  Implicit Types a : socket_address.
-  Implicit Types ip : ip_address.
-  Implicit Types sh : socket_handle.
-  Implicit Types skt : socket.
-  Implicit Types A B : gset socket_address.
-  Implicit Types pms : gmap port (message_soup * message_soup).
-  Implicit Types mhγ : gmap ip_address (gmap port (message_soup * message_soup)).
-  Implicit Types γm : gmap ip_address node_gnames.
-  Implicit Types sis : gmap socket_address gname.
-
-  (* The local state of the node at [ip] is coherent with [σ] and [γs] *)
-  Definition local_state_coh σ ip γs :=
-    (∃ h Sn,
-        ⌜state_heaps σ !! ip = Some h⌝ ∗
-        ⌜state_sockets σ !! ip = Some Sn⌝ ∗
-        mapsto_node ip γs ∗
-        heap_ctx γs h ∗
-        sockets_ctx γs Sn)%I.
-
-  (*Definition gset_ipofsa := gset_map ip_of_address.
-
-  Definition messages_history_new_node ip ps mhγ :=
-   set_fold (fun p acc => <[(SocketAddressInet ip p):=(∅, ∅)]> acc) mhγ ps.*)
-
-  (** The domains of heaps and sockets coincide with the gname map [γm] *)
-  Definition gnames_coh γm H S mhγ :=
-    dom (gset ip_address) γm = dom (gset ip_address) H ∧
-    dom (gset ip_address) γm = dom (gset ip_address) S ∧
-    dom (gset ip_address) γm = dom (gset ip_address) mhγ.
-
-  (* Addresses with socket interpretations are bound *)
-  Definition socket_interp_coh P :=
-    (∃ sis A,
-        (* [A] is the set of addresses with fixed interpretations *)
-        fixed A ∗
-        (* [si] is the map from addresses to name of
-           saved socket interpretations *)
-        saved_si_auth sis ∗
-        (* there exists a socket interpretation for all addresses in this map *)
-        ([∗ set] s ∈ (dom (gset socket_address) sis), ∃ φ, s ⤇ φ) ∗
-        (* the addresses in A are in the domain of P *)
-        ⌜∀ a, a ∈ A → ip_of_address a ∈ dom (gset ip_address) P⌝ ∗
-        (* all addresses in [si] either have a fixed interpretation ([a ∈ A]) or
-           are dynamically bound. *)
-        ⌜∀ a, (ip_of_address a ∈ dom (gset ip_address) P) →
-              (a ∈ dom (gset socket_address) sis ↔
-                 a ∈ A ∨ (a ∉ A ∧ ∀ ps, P !! ip_of_address a = Some ps →
-                                        port_of_address a ∈ ps))⌝)%I.
-
-  (* Free ips have no bound ports, no heap, and no sockets  *)
-  Definition free_ips_coh σ :=
-    (∃ free_ips free_ports,
-        (* the domains of [free_ips] and [free_ports] are disjoint *)
-        (⌜dom (gset _) free_ports ## free_ips ∧
-         (* if the ip [ip] is free, no ports have been bound  *)
-         (∀ ip, ip ∈ free_ips → state_ports_in_use σ !! ip = Some ∅) ∧
-         (* if the ip [ip] is free, neither a heap nor a socket map has been
-            allocated *)
-         (∀ ip, ip ∈ free_ips →
-                state_heaps σ !! ip = None ∧ state_sockets σ !! ip = None) ∧
-         (* free ports and bound ports are disjoint *)
-         (∀ ip ps, free_ports !! ip = Some (GSet ps) →
-             ∃ bound_ports,
-               (state_ports_in_use σ) !! ip = Some bound_ports ∧
-               ps ## bound_ports )⌝) ∗
-         (* we have the auth parts of the resources for free ips and ports *)
-         free_ips_auth free_ips ∗
-         free_ports_auth free_ports)%I.
-
-  (* The ports of all bound addresses in [Sn] are also in [P] *)
-  Definition bound_ports_coh Sn P :=
-    ∀ sh skt a ps r,
-      Sn !! sh = Some (skt, r) →
-      saddress skt = Some a →
-      P !! ip_of_address a = Some ps →
-      (port_of_address a) ∈ ps.
-
-  (* All sockets in [Sn] with the same address have the same handler *)
-  Definition socket_handlers_coh Sn :=
-    ∀ sh sh' skt skt' r r',
-      Sn !! sh = Some (skt, r) →
-      Sn !! sh' = Some (skt', r') →
-      is_Some (saddress skt) →
-      saddress skt = saddress skt' →
-      sh = sh'.
-
-  (* Sent and received messages at all socket in [Sn] are in [M] *)
-  Definition socket_messages_coh Sn :=
-    ∀ sh skt r a,
-      Sn !! sh = Some (skt, r) →
-      saddress skt = Some a →
-      ∀ m, m ∈ r → m_destination m = a.
-
-  (* all sockets in [Sn] are bound to ip address [ip] *)
-  Definition socket_addresses_coh Sn ip :=
-    ∀ sh skt r a,
-      Sn !! sh = Some (skt, r) →
-      saddress skt = Some a →
-      ip_of_address a = ip.
-
-  Definition network_sockets_coh S P :=
-    ∀ ip Sn,
-      S !! ip = Some Sn →
-      bound_ports_coh Sn P ∧
-      socket_handlers_coh Sn ∧
-      socket_messages_coh Sn ∧
-      socket_addresses_coh Sn ip.
-
-  Definition get_address_messages mhγ sa :=
-    match (mhγ !! (ip_of_address sa)) with
-    | None => (∅, ∅)
-    | Some mps =>
-      match mps !! (port_of_address sa) with
-      | None => (∅, ∅)
-      | Some (R,T) => (R,T)
-      end
-    end.
-
-  (* Definition get_message_history mhγ sa := *)
-  (*   pms ← (mhγ !! (ip_of_address sa)); pms !! (port_of_address sa). *)
-
-
-  Definition message_soup_coh M mhγ :=
-    ∀ m, m ∈ M →
-         ∃ R T, get_address_messages mhγ (m_sender m) = (R, T) ∧ m ∈ T.
-
-  Definition receive_buffers_coh S mhγ :=
-    ∀ ip Sn sh skt r m,
-      S !! ip = Some Sn →
-      Sn !! sh = Some (skt, r) → m ∈ r →
-      ∃ R T, get_address_messages mhγ (m_sender m) = (R, T) ∧ m ∈ T.
-
-  Definition messages_addresses_coh mhγ :=
-    ∀ a R T, get_address_messages mhγ a = (R, T) →
-             (∀ m, m ∈ R → m_destination m = a) ∧
-             (∀ m, m ∈ T → m_sender m = a).
-
-  Definition messages_history_coh M S mhγ :=
-    message_soup_coh M mhγ ∧
-    receive_buffers_coh S mhγ ∧
-    messages_addresses_coh mhγ.
-
-  (* Received messages *)
-  Definition messages_received mhγ :=
-    map_fold (fun ip pms acc0 =>
-                map_fold (fun p rt acc1 => rt.1 ∪ acc1) acc0 pms) ∅ mhγ.
-
-  Definition messages_sent mhγ :=
-    map_fold (fun ip pms acc0 =>
-                map_fold (fun p rt acc1 => rt.2 ∪ acc1) acc0 pms) ∅ mhγ.
-
-  (* [m] has been received *)
-  Definition message_received m mhγ := m ∈ (messages_received mhγ).
-
-  Definition messages_init (ports : gset port) :=
-    set_fold (fun p macc => <[p := (∅, ∅)]>macc)
-             (∅: gmap port (message_soup * message_soup)) ports.
-
- (* For all messages [m] in [M], either the network owns the resources [Φ m]
-     described by some socket protocol [Φ] or it has been delivered *)
-  Definition messages_resource_coh mhγ :=
-    ([∗ set] m ∈ messages_sent mhγ,
-     (* either [m] is governed by a protocol and
-        the network owns the resources *)
-     (∃ (Φ : socket_interp Σ), (m_destination m) ⤇ Φ ∗ ▷ Φ m) ∨
-     (* or [m] has been delivered somewhere *)
-     ⌜message_received m mhγ⌝)%I.
-
-  Definition aneris_state_interp σ :=
-    (∃ γm mhγ,
-        ⌜gnames_coh γm (state_heaps σ) (state_sockets σ) mhγ⌝ ∗
-        ⌜network_sockets_coh (state_sockets σ) (state_ports_in_use σ)⌝ ∗
-        ⌜messages_history_coh (state_ms σ) (state_sockets σ) mhγ⌝ ∗
-        node_gnames_auth γm ∗
-        socket_interp_coh (state_ports_in_use σ) ∗
-        ([∗ map] ip ↦ γs ∈ γm, local_state_coh σ ip γs) ∗
-        free_ips_coh σ ∗
-        messages_ctx mhγ ∗
-        messages_resource_coh mhγ)%I.
-
-End definitions.
-
-
-Global Instance anerisG_irisG `{!anerisG Σ} : irisG aneris_lang Σ := {
-  iris_invG := _;
-  state_interp σ κ _ := aneris_state_interp σ;
-  fork_post _ := True%I;
-}.
-
-Global Opaque iris_invG.
-
 Section state_interpretation.
   Context `{!anerisG Σ}.
-
-  (** local_state_coh *)
-  Lemma local_state_coh_heaps n γs γm σ :
-    γm !! n = Some γs →
-    ([∗ map] n' ↦ γs ∈ γm, local_state_coh σ n' γs) -∗
-    ∃ h, ⌜(state_heaps σ) !! n = Some h⌝.
-  Proof.
-    iIntros (?) "Hmap".
-    iDestruct (big_sepM_lookup with "Hmap") as "Hl"; [done|].
-    iDestruct "Hl" as (????) "_"; eauto.
-  Qed.
-
-  Lemma local_state_coh_sockets n γs γm σ :
-    γm !! n = Some γs →
-    ([∗ map] n' ↦ γs ∈ γm, local_state_coh σ n' γs) -∗
-    ∃ Sn, ⌜(state_sockets σ) !! n = Some Sn⌝.
-  Proof.
-    iIntros (?) "Hmap".
-    iDestruct (big_sepM_lookup with "Hmap") as "Hl"; [done|].
-    iDestruct "Hl" as (????) "_"; eauto.
-  Qed.
-
-  Lemma local_state_coh_alloc_heap σ n γs l v h :
-    let σ' := σ <| state_heaps := <[n:=<[l:=v]> h]> (state_heaps σ) |> in
-    state_heaps σ !! n = Some h →
-    h !! l = None →
-    is_node n -∗
-    local_state_coh σ n γs ==∗ local_state_coh σ' n γs ∗ l ↦[n] v.
-  Proof.
-    simpl. iIntros (??) "Hn Hstate". iDestruct "Hn" as (?) "#Hn".
-    iDestruct "Hstate" as (h' S Hh Hs) "(Hn' & Hheap & ?)".
-    iDestruct (mapsto_node_agree with "Hn Hn'") as %->.
-    simplify_eq.
-    iMod (gen_heap_light_alloc with "Hheap") as "[Hheap Hl]"; [done|].
-    iModIntro. iFrame.
-    iSplitR "Hl"; [| iExists _; eauto].
-    iExists _, _. iFrame.
-    rewrite lookup_insert //.
-  Qed.
-
-  Lemma local_state_coh_valid_heap σ n γs l v q :
-    local_state_coh σ n γs -∗
-    l ↦[n]{q} v -∗
-    ∃ h, ⌜state_heaps σ !! n = Some h ∧ h !! l = Some v⌝.
-  Proof.
-    iDestruct 1 as (h' S Hh Hs) "(Hn & Hheap & Hsock)".
-    iDestruct 1 as (γs') "[Hn' Hl]".
-    iDestruct (mapsto_node_agree with "Hn Hn'") as %->.
-    iDestruct (gen_heap_light_valid with "Hheap Hl") as "%".
-    iExists _. iPureIntro; eauto.
-  Qed.
-
-  Lemma local_state_coh_update_heap σ1 n γs h l v1 v2 :
-    let σ2 := (σ1 <| state_heaps := <[n:=<[l:=v2]> h]> (state_heaps σ1) |>) in
-    state_heaps σ1 !! n = Some h →
-    local_state_coh σ1 n γs ∗ l ↦[n] v1 ==∗ local_state_coh σ2 n γs ∗ l ↦[n] v2.
-  Proof.
-    simpl. iIntros (?) "[Hstate Hl]".
-    iDestruct "Hstate" as (h' Sn Hh Hs) "(#Hn & Hheap & ?)".
-    iDestruct "Hl" as (γs') "[Hn' Hl]".
-    iDestruct (mapsto_node_agree with "Hn Hn'") as %->.
-    simplify_eq.
-    iMod (gen_heap_light_update with "Hheap Hl") as "[Hheap' Hl]".
-    iModIntro. iFrame.
-    iSplitR "Hl"; [| iExists _; eauto].
-    iExists _, _. iFrame.
-    rewrite lookup_insert /set /=; eauto.
-  Qed.
-
-  Lemma local_state_coh_valid_sockets σ ip γs sh q skt :
-    local_state_coh σ ip γs -∗
-    sh ↪[ip]{q} skt -∗
-    ∃ Sn r, ⌜state_sockets σ !! ip = Some Sn ∧ Sn !! sh = Some (skt, r)⌝.
-  Proof.
-    iDestruct 1 as (h' Sn Hh Hs) "(Hn & Hh & Hs)".
-    rewrite mapsto_socket_eq.
-    iDestruct 1 as (γs' r) "[Hn' Hsh]".
-    iDestruct (mapsto_node_agree with "Hn Hn'") as %->.
-    iDestruct (gen_heap_light_valid with "Hs Hsh") as "%Hfd".
-    iExists _, _. iPureIntro; eauto.
-  Qed.
-
-  Lemma local_state_coh_alloc_socket σ ip γs sh Sn skt:
-    let σ' := σ <| state_sockets :=
-                <[ip:=<[sh:=(skt, ∅)]> Sn]> (state_sockets σ)|> in
-    state_sockets σ !! ip = Some Sn →
-    Sn !! sh = None →
-    is_node ip -∗
-    local_state_coh σ ip γs ==∗
-    local_state_coh σ' ip γs ∗ sh ↪[ip] skt.
-  Proof.
-    simpl. iIntros (??) "Hn Hstate". iDestruct "Hn" as (?) "#Hn".
-    iDestruct "Hstate" as (h' Sn' Hh Hs) "(Hn' & Hh & Hs)".
-    iDestruct (mapsto_node_agree with "Hn Hn'") as %->.
-    simplify_eq.
-    iMod (gen_heap_light_alloc _ sh _ _  with "Hs") as "[Hsock Hsh]"; [done|].
-    iModIntro. iFrame.
-    rewrite mapsto_socket_eq.
-    iSplitR "Hsh"; [|iExists _, _; eauto].
-    iExists _, _; eauto. iFrame.
-      rewrite lookup_insert //.
-  Qed.
-
-  Lemma local_state_coh_socketbind σ1 γs sh skt a Sn ps :
-    let ip := ip_of_address a in
-    let S' :=
-        <[ip :=
-            <[sh:=(skt<| saddress := Some a |>, ∅)]> Sn]> (state_sockets σ1) in
-    let P' := <[ip := {[port_of_address a]} ∪ ps]> (state_ports_in_use σ1) in
-    let σ2 := σ1 <| state_sockets := S' |> <| state_ports_in_use := P' |> in
-    state_sockets σ1 !! ip = Some Sn →
-    Sn !! sh = Some (skt, ∅) →
-    state_ports_in_use σ1 !! ip = Some ps →
-    saddress skt = None →
-    local_state_coh σ1 ip γs ∗ sh ↪[ip] skt ==∗
-    local_state_coh σ2 ip γs ∗ sh ↪[ip] (skt<| saddress := Some a |>).
-  Proof.
-    simpl. iIntros (????) "[Hlcoh Hsh]".
-    iDestruct "Hlcoh" as (h' S Hh Hs) "(#Hn & ? & Hsock)".
-    rewrite mapsto_socket_eq.
-    iDestruct "Hsh" as (γs' r) "[Hn' Hsh]".
-    iDestruct (mapsto_node_agree with "Hn Hn'") as %<-.
-    simplify_eq.
-    iMod (gen_heap_light_update _ _ _ _ (skt<| saddress := Some a |>, ∅)
-            with "Hsock Hsh") as "[Hsock' Hsh]".
-    iModIntro. iFrame.
-    iSplitR "Hsh"; [| iExists _; eauto].
-    iExists _, _. iFrame.
-    rewrite lookup_insert /set /=; eauto.
-  Qed.
-
-  Lemma local_state_coh_update_rb a sh skt σ1 γs Sn r r' :
-    let ip := ip_of_address a in
-    let S' := <[ip := <[sh:=(skt, r')]> Sn]> (state_sockets σ1) in
-    let σ2 := σ1 <| state_sockets := S' |> in
-    state_sockets σ1 !! ip = Some Sn →
-    Sn !! sh = Some (skt, r) →
-    local_state_coh σ1 ip γs ∗ sh ↪[ip] skt ==∗
-    local_state_coh σ2 ip γs ∗ sh ↪[ip] skt.
-  Proof.
-    iIntros (?????) "[Hstate Hsh]".
-    iDestruct "Hstate" as (h' S Hh Hs) "(#Hn & ? & Hsock)".
-    rewrite mapsto_socket_eq.
-    iDestruct "Hsh" as (γs' r0) "[Hn' Hsh]".
-    iDestruct (mapsto_node_agree with "Hn Hn'") as %->.
-    simplify_eq.
-    iMod (gen_heap_light_update _ _ _ _ (skt, r')
-            with "Hsock Hsh") as "[Hsock' Hsh]".
-    iModIntro. iFrame. iSplitR "Hsh".
-    { iExists _, _. iFrame. rewrite lookup_insert //. }
-    iExists _; eauto.
-  Qed.
-
-  Lemma big_sepM_local_state_coh_insert n γs γm σ :
-    γm !! n = Some γs →
-    local_state_coh σ n γs -∗
-    ([∗ map] n' ↦ x ∈ delete n γm, local_state_coh σ n' x) -∗
-    [∗ map] n' ↦ x ∈ γm, local_state_coh σ n' x.
-  Proof.
-    iIntros (Hlookup%insert_id) "Hl Hmap".
-    iDestruct (big_sepM_insert with "[$]") as "HP".
-    { apply lookup_delete. }
-    rewrite insert_delete Hlookup //.
-  Qed.
-
-  Lemma big_sepM_local_state_coh_delete n γs γm σ :
-    γm !! n = Some γs →
-    ([∗ map] n' ↦ x ∈ γm, local_state_coh σ n' x) -∗
-    local_state_coh σ n γs ∗
-    [∗ map] n' ↦ x ∈ delete n γm, local_state_coh σ n' x.
-  Proof. iIntros (?) "?"; rewrite -big_sepM_delete //. Qed.
-
-
-  Lemma big_sepM_local_state_coh_alloc_node n γm σ :
-    γm !! n = None →
-    ([∗ map] n' ↦ x ∈ γm, local_state_coh σ n' x) -∗
-    [∗ map] n' ↦ x ∈ γm,
-    local_state_coh (σ <| state_heaps   := <[n:=∅]> (state_heaps σ)|>
-                       <| state_sockets := <[n:=∅]> (state_sockets σ) |>) n' x.
-  Proof.
-    intros ?.
-    rewrite big_sepM_mono; [done|].
-    intros n' x Hdel.
-    destruct (decide (n = n')); simplify_eq.
-    rewrite /local_state_coh !lookup_insert_ne //.
-  Qed.
-
-  Lemma big_sepM_local_state_coh_update_heap_notin n γm σ1 h :
-    let σ2 := (σ1 <| state_heaps := <[n:=h]>(state_heaps σ1) |>) in
-    γm !! n = None →
-    ([∗ map] n' ↦ x ∈ γm, local_state_coh σ1 n' x) -∗
-    [∗ map] n' ↦ x ∈ γm, local_state_coh σ2 n' x.
-  Proof.
-    simpl. intros ?.
-    rewrite big_sepM_mono; [done|].
-    intros n' x Hdel.
-    destruct (decide (n = n')); simplify_eq.
-    rewrite /local_state_coh lookup_insert_ne //.
-  Qed.
-
-
-  Lemma big_sepM_local_state_coh_update_socket_notin n γm Sn σ1 :
-    let σ2 := (σ1 <| state_sockets := <[n:=Sn]>(state_sockets σ1) |>) in
-    γm !! n = None →
-    ([∗ map] n' ↦ x ∈ γm, local_state_coh σ1 n' x) -∗
-    [∗ map] n' ↦ x ∈ γm, local_state_coh σ2 n' x.
-  Proof.
-    simpl. intros ?.
-    rewrite big_sepM_mono; [done|].
-    intros n' x Hdel.
-    destruct (decide (n = n')); simplify_eq.
-    rewrite /local_state_coh lookup_insert_ne //.
-  Qed.
-
-  (** gnames_coh *)
-  (* TODO: check whether this works out. *)
-  Lemma gnames_coh_singleton_empty ip γs :
-    gnames_coh {[ip:=γs]} {[ip:=∅]} {[ip:=∅]} {[ip:=∅]}.
-  Proof. rewrite /gnames_coh !dom_singleton_L //. Qed.
-
-  Lemma gnames_coh_singleton ip γs h Sn p R T:
-    gnames_coh {[ip:=γs]} {[ip:=h]} {[ip:=Sn]} {[ip:= {[p:=(R,T)]} ]}.
-  Proof. rewrite /gnames_coh !dom_singleton_L //. Qed.
-
-  Lemma gnames_coh_valid γm H S ip Mγ :
-    H !! ip = None →
-    gnames_coh γm H S Mγ →
-    γm !! ip = None.
-  Proof. rewrite -!not_elem_of_dom => _ [-> _] //. Qed.
-
-  Lemma gnames_coh_alloc_node γm H S ip γn mhγ ports:
-    gnames_coh γm H S mhγ →
-    gnames_coh (<[ip:=γn]> γm) (<[ip:=∅]> H) (<[ip:=∅]> S)
-               (<[ip:= messages_init ports]> mhγ).
-  Proof. rewrite /gnames_coh !dom_insert_L.
-         move=> [->] //=. set_solver.
-  Qed.
-
-  Lemma gnames_coh_update_heap n γm H S h h' Mγ:
-    H !! n = Some h →
-    gnames_coh γm H S Mγ →
-    gnames_coh γm (<[n:=h']> H) S Mγ.
-  Proof.
-    intros ?%elem_of_dom_2 [? ?].
-    rewrite /gnames_coh dom_insert_L subseteq_union_1_L //=.
-    set_solver.
-  Qed.
-
-  Lemma gnames_coh_update_sockets n γm H S Sn Sn' Mγ :
-    S !! n = Some Sn →
-    gnames_coh γm H S Mγ →
-    gnames_coh γm H (<[n:=Sn']> S) Mγ.
-  Proof.
-    intros ?%elem_of_dom_2 [? ?].
-    rewrite /gnames_coh dom_insert_L subseteq_union_1_L //=.
-    set_solver.
-  Qed.
-
-  (** free_ips_coh *)
-  Lemma free_ips_coh_init ip ips σ :
-    ip ∉ ips →
-    dom (gset ip_address) (state_ports_in_use σ) = ips →
-    (∀ ip, ip ∈ ips → state_ports_in_use σ !! ip = Some ∅) →
-    state_heaps σ = {[ip:=∅]} →
-    state_sockets σ = {[ip:=∅]} →
-    state_ms σ = ∅ →
-    free_ips_auth ips ∗ free_ports_auth ∅ -∗ free_ips_coh σ.
-  Proof.
-    iIntros (??? Hste Hsce ?) "[HipsCtx HPiu]".
-    iExists _, _; iFrame.
-    rewrite Hste Hsce.
-    iPureIntro.
-    do 2 (split; [set_solver|]).
-    split; [|set_solver].
-    intros ip' ?.
-    assert (ip ≠ ip') by set_solver.
-    rewrite !lookup_insert_ne //.
-  Qed.
-
-  Lemma free_ips_coh_free_ports_valid σ a :
-    free_ips_coh σ -∗
-    free_ports (ip_of_address a) {[port_of_address a]} -∗
-    ∃ ps, ⌜state_ports_in_use σ !! ip_of_address a = Some ps ∧
-           port_of_address a ∉ ps⌝.
-  Proof.
-    iDestruct 1 as (Fip Piu (Hdsj & HFip & HFip2 & HPiu)) "[HfCtx HpCtx]".
-    iIntros "Hp".
-    iDestruct (free_ports_included with "HpCtx Hp") as (?) "[%Hlookup %]".
-    destruct (HPiu _ _ Hlookup) as (?&?&?).
-    iExists _. iPureIntro. split; [done|set_solver].
-  Qed.
-
-  Lemma free_ips_coh_alloc_node σ ip ports :
-    free_ips_coh σ -∗
-    free_ip ip ==∗
-    free_ips_coh (σ <| state_heaps   := <[ip:=∅]> (state_heaps σ)|>
-                    <| state_sockets := <[ip:=∅]> (state_sockets σ) |>) ∗
-    free_ports ip ports.
-  Proof.
-    iDestruct 1 as (Fip Piu (Hdsj & HFip & HFip2 & HPiu)) "[HfCtx HpCtx]".
-    iIntros "Hfip".
-    iDestruct (free_ip_included with "HfCtx Hfip") as %Hin.
-    iMod (free_ip_dealloc with "HfCtx Hfip") as "HfCtx".
-    iMod (free_ports_alloc _ ip ports with "HpCtx") as "[HpCtx Hports]";
-      [set_solver|].
-    iModIntro. iFrame. iExists _, _. simpl. iFrame. iPureIntro.
-    split; [set_solver|]. split; [set_solver|]. split.
-    { intros. rewrite !lookup_insert_ne //; set_solver. }
-    intros ip' ??.
-    destruct (decide (ip = ip')); simplify_map_eq; [|eauto].
-    eexists; split; eauto. set_solver.
-  Qed.
-
-  Lemma free_ips_coh_update_heap σ ip h h' :
-    state_heaps σ !! ip = Some h →
-    free_ips_coh σ -∗
-    free_ips_coh (σ <| state_heaps := <[ip:=h']> (state_heaps σ) |>).
-  Proof.
-    iIntros (?).
-    iDestruct 1 as (Fip Piu (Hdsj & HFip & HFip2 & HPiu)) "[HfCtx HpCtx]".
-    iExists _, _. simpl. iFrame. iPureIntro.
-    do 3 (split; auto).
-    intros ip' ?.
-    split; [|set_solver].
-    destruct (decide (ip = ip')); simplify_map_eq; [set_solver|].
-    by apply HFip2.
-  Qed.
-
-  Lemma free_ips_coh_alloc_socket σ ip Sn sh sock :
-    let σ' :=
-        σ <| state_sockets := <[ip:=<[sh:=sock]> Sn]> (state_sockets σ) |> in
-    state_sockets σ !! ip = Some Sn →
-    Sn !! sh = None →
-    free_ips_coh σ -∗ free_ips_coh σ'.
-  Proof.
-    iIntros (???).
-    iDestruct 1 as (Fip Piu (Hdsj & HFip & HFip2 & HPiu)) "[HfCtx HpCtx]".
-    iExists _, _. simpl. iFrame. iPureIntro.
-    do 3 (split; auto).
-    intros ip' ?.
-    split; [by eapply HFip2|].
-    destruct (decide (ip = ip')); simplify_map_eq; [set_solver|].
-    by apply HFip2.
-  Qed.
-
-  Lemma free_ips_coh_dealloc σ1 a sh skt Sn ps :
-    let ip := ip_of_address a in
-    let S' := <[ip := <[sh:=(skt<| saddress := Some a |>, ∅)]> Sn]>
-              (state_sockets σ1) in
-    let P' := <[ip := {[port_of_address a]} ∪ ps]> (state_ports_in_use σ1) in
-    let σ2 := σ1 <| state_sockets := S' |> <| state_ports_in_use := P' |> in
-    state_sockets σ1 !! ip = Some Sn →
-    state_ports_in_use σ1 !! ip = Some ps →
-    free_ips_coh σ1 -∗
-    free_ports (ip_of_address a) {[port_of_address a]} ==∗
-    free_ips_coh σ2.
-  Proof.
-    rewrite /free_ips_coh /=.
-    iDestruct 1 as (Fip Piu (Hdsj & HFip & HFip2 & HPiu)) "[HfCtx HpCtx]".
-    iIntros "Hp".
-    iMod (free_ports_dealloc with "HpCtx Hp")
-               as (ps' [Hps' Hin%elem_of_subseteq_singleton]) "HpCtx".
-    iModIntro. iExists _, _; iFrame. iPureIntro.
-    split; [set_solver|].
-    split.
-    { intros ip ?.
-      destruct (decide (ip = ip_of_address a)); simplify_eq; [set_solver|].
-      rewrite lookup_insert_ne //. by apply HFip. }
-    split.
-    { intros ip ?. split; [set_solver|].
-      destruct (decide (ip = ip_of_address a)); simplify_eq; [set_solver|].
-      rewrite lookup_insert_ne //. by apply HFip2. }
-    intros ip ??.
-    destruct (decide (ip = ip_of_address a)); simplify_map_eq.
-    - destruct (HPiu _ _ Hps') as [Q [Ha HQ]]. simplify_map_eq.
-      eexists. split; [done|]. set_solver.
-    - rewrite lookup_insert_ne //. set_solver.
-  Qed.
-
-  Lemma free_ips_coh_update_msg sh a skt Sn r' σ1 :
-    let ip := ip_of_address a in
-    let S' := <[ip := <[sh:=(skt, r')]> Sn]> (state_sockets σ1) in
-    let σ2 := σ1 <| state_sockets := S' |> in
-    state_sockets σ1 !! ip_of_address a = Some Sn →
-    Sn !! sh = Some (skt, r') →
-    free_ips_coh σ1 -∗ free_ips_coh σ2.
-  Proof.
-    rewrite /free_ips_coh /=.
-    iDestruct 1 as (Fip Piu (Hdsj & HFip & HFip2 & HPiu)) "[HfCtx HpCtx]".
-    iExists _, _. simpl. iFrame. iPureIntro.
-    do 2 (split; [auto|]).
-    split; [|done].
-    intros ip ?. split; [set_solver|].
-    destruct (decide (ip = ip_of_address a)); simplify_map_eq; [set_solver|].
-    by apply HFip2.
-  Qed.
-
-
-  (** message_received *)
-  (* TODO: FIXME *)
-  (*
-  Lemma message_received_alloc_socket S m Sn ip sh s:
-    S !! ip = Some Sn →
-    Sn !! sh = None →
-    message_received S m →
-    message_received (<[ip:=<[sh:=(s, ∅, ∅)]> Sn]> S) m.
-  Proof.
-    rewrite /message_received.
-    intros HSn HhNone (Sn' & sh' & s' & a & R & T & HS' & HSn' & Ha & Hm).
-    destruct (decide (ip = ip_of_address a)); simplify_map_eq.
-    - eexists  (<[sh:=(s, ∅, ∅)]> Sn), _, _, a, _, _.
-      rewrite lookup_insert. repeat split; try done.
-      rewrite lookup_insert_ne //.
-    - do 6 eexists. rewrite lookup_insert_ne //.
-  Qed.
-
-  Lemma message_received_socketbind S m Sn sh skt a:
-    let ip := ip_of_address a in
-    let S' := (<[ip:=<[sh:=(skt <| saddress := Some a |>, ∅, ∅)]> Sn]> S) in
-    S !! ip = Some Sn →
-    Sn !! sh = Some (skt, ∅, ∅) →
-    message_received S m →
-    message_received S' m.
-  Proof.
-    rewrite /message_received.
-    intros HSn HhSome (? & sh' &?& a' &?&?&HS&?&?&?).
-    destruct (decide (ip_of_address a = ip_of_address a')) as [Heq|];
-      simplify_map_eq.
-    - rewrite -Heq in HS.
-      destruct (decide (sh = sh')); simplify_map_eq; [done|].
-      eexists (<[sh:=(skt<| saddress := Some a |>, ∅, ∅)]> Sn), _, _, a',  _, _.
-      rewrite Heq lookup_insert lookup_insert_ne //.
-    - do 6 eexists. rewrite lookup_insert_ne //.
-  Qed.
-
-  Lemma message_received_receive a skt sh S Sn R T m :
-    let S' := (<[ip_of_address a:=<[sh:=(skt, {[m]} ∪ R, T)]> Sn]> S) in
-    S !! ip_of_address a = Some Sn →
-    Sn !! sh = Some (skt, R, T) →
-    saddress skt = Some a →
-    message_received S' m.
-  Proof.
-    intros ????. rewrite /message_received /S'.
-    exists (<[sh:=(skt, {[m]} ∪ R, T)]> Sn), sh, skt, a, ({[m]} ∪ R), T.
-    rewrite !lookup_insert //. repeat split; eauto. set_solver.
-  Qed.
-
-  Lemma message_received_insert a skt sh S Sn R T m m' :
-    let S' := (<[ip_of_address a:=<[sh:=(skt, {[m']} ∪ R, T)]> Sn]> S) in
-    S !! ip_of_address a = Some Sn →
-    Sn !! sh = Some (skt, R, T) →
-    saddress skt = Some a →
-    message_received S m →
-    message_received S' m.
-  Proof.
-    intros S' HS HSn ? Hr.
-    destruct (decide (m = m')); simplify_eq.
-    { by apply message_received_receive. }
-    destruct Hr as (Sn' & sh' & skt' & a' & R' & T' & HS' & HSn' & Ha' & Hm).
-    rewrite /S' /message_received.
-    destruct (decide (ip_of_address a = ip_of_address a')) as [Heq | ?].
-    - exists (<[sh:=(skt, {[m']} ∪ R, T)]> Sn).
-      rewrite -Heq in HS'.
-      assert (Sn = Sn') as <- by set_solver.
-      destruct (decide (sh' = sh)); simplify_eq.
-      + exists sh, skt, a, ({[m']} ∪ R), T.
-        rewrite !lookup_insert. repeat split; eauto with set_solver.
-      + exists sh', skt', a', R', T'.
-        rewrite Heq ?lookup_insert ?lookup_insert_ne //.
-    - do 6 eexists. rewrite lookup_insert_ne //.
-   Qed.
-   *)
-
-  (* TODO: FIXME *)
-  (*
-  (** network_messages_coh *)
-  Lemma network_messages_coh_alloc_node Sn M ip :
-    Sn !! ip = None →
-    network_messages_coh Sn M -∗
-    network_messages_coh (<[ip:=∅]> Sn) M.
-  Proof.
-    iIntros (Hnone) "H".
-    iApply big_sepS_mono; last done.
-    iIntros (??) "[? | %Hr]"; first by iLeft.
-    destruct Hr as (a & h & Sn' & s & R & T &?&?&?&?).
-    iRight. iPureIntro. exists a, h, Sn', s, R, T.
-    simplify_map_eq. set_solver.
-  Qed.
-
-  Lemma network_messages_coh_alloc_socket S Sn M n h sh :
-    S !! n = Some Sn →
-    Sn !! h = None →
-    network_messages_coh S M -∗
-    network_messages_coh (<[n:=<[h:=(sh, ∅, ∅)]>Sn]> S) M.
-  Proof.
-    iIntros (??) "Hsent". rewrite /network_messages_coh.
-    rewrite big_sepS_mono; first done.
-    iIntros (??) "[Htt | %]"; [by iLeft|].
-    iRight. iPureIntro. by apply message_received_alloc_socket.
-  Qed.
-
-  Lemma network_messages_coh_socketbind S M Sn sh skt a :
-    let ip := ip_of_address a in
-    let S' := (<[ip:=<[sh:=(skt <| saddress := Some a |>, ∅, ∅)]> Sn]> S) in
-    S !! ip = Some Sn →
-    Sn !! sh = Some (skt, ∅, ∅) →
-    saddress skt = None →
-    network_messages_coh S M -∗
-    network_messages_coh S' M.
-  Proof.
-    rewrite /network_messages_coh /=.
-    iIntros (???) "Hsent".
-    rewrite big_sepS_mono; first done.
-    iIntros (??) "[? | %]"; [by iLeft|].
-    iRight. iPureIntro. by apply message_received_socketbind.
-  Qed.
-
-  Lemma network_messages_coh_insert_sent S M Sn sh skt a to m R T φ P :
-    let ip := ip_of_address a in
-    let msg := mkMessage a to (sprotocol skt) m in
-    let S' := <[ip := <[sh:=(skt, R, {[msg]} ∪ T)]> Sn]> S in
-    let M' := {[msg]} ∪ M in
-    saddress skt = Some a →
-    S !! ip = Some Sn →
-    Sn !! sh = Some (skt, R, T) →
-    network_sockets_coh S M P →
-    to ⤇ φ -∗
-    φ msg -∗
-    network_messages_coh S M -∗ network_messages_coh S' M'.
-  Proof.
-    iIntros (ip msg ?? Hsa Hh Hsi HnetCoh) "Hsi Hmsg Hsent".
-    rewrite /network_messages_coh /S'.
-    destruct (decide (msg ∈ M)).
-    - assert (M = M') as <- by set_solver.
-      iApply (big_sepS_mono with "Hsent").
-      iIntros (msg' Hmsg') "[Htt | Hrd]"; first by iLeft.
-      iDestruct "Hrd" as %Hrd. iRight; iPureIntro.
-      rewrite /message_received.
-      destruct Hrd as (Sa'&sh'&skt'&a'&R'&T'&Hsi'&Hs'&Hsa'&HinR').
-      destruct (decide (ip = ip_of_address a')) as [Heq | Heq]; simplify_map_eq.
-      + eexists (<[sh:=(skt, R, {[msg]} ∪ T)]> Sn),sh',skt',a'.
-        destruct Heq.
-        destruct (decide (sh = sh')); do 2 eexists;
-          simplify_map_eq; [done|].
-        rewrite lookup_insert_ne //.
-      + do 6 eexists. rewrite lookup_insert_ne //.
-    - rewrite (big_sepS_union _ _ M ) // /=; last by set_solver.
-      iSplitL "Hmsg Hsi". rewrite big_sepS_singleton. iLeft. eauto.
-      iApply (big_sepS_mono with "Hsent").
-      iIntros (msg' Hmsg') "[Htt | Hrd]"; first by iLeft.
-      iDestruct "Hrd" as %Hrd. iRight; iPureIntro.
-      rewrite /message_received.
-      destruct Hrd as (Sa'&sh'&skt'&a'&R'&T'&Hsi'&Hs'&Hsa'&HinR').
-      destruct (decide (ip = ip_of_address a')) as [Heq | Heq]; simplify_map_eq.
-      + eexists (<[sh:=(skt, R, {[msg]} ∪ T)]> Sn),sh',skt',a'.
-        destruct Heq. rewrite lookup_insert.
-        destruct (decide (sh = sh')); do 2 eexists;
-          simplify_map_eq; [done|].
-        rewrite lookup_insert_ne //.
-      + do 6 eexists. rewrite lookup_insert_ne //.
-  Qed.
-*)
-
-  (** bound_ports_coh *)
-  Lemma bound_ports_coh_alloc_socket Sn P sh skt :
-    Sn !! sh = None →
-    saddress skt = None →
-    bound_ports_coh Sn P →
-    bound_ports_coh (<[sh:=(skt, ∅)]> Sn) P.
-  Proof.
-    intros ??? sh' ???? Hup.
-    destruct (decide (sh = sh')) as [Heq|];
-      simplify_map_eq.
-    - rewrite lookup_insert in Hup. simplify_eq /=.
-      intros. simplify_eq /=.
-    - rewrite lookup_insert_ne in Hup; eauto.
-  Qed.
-
-
-  Lemma bound_ports_coh_socketbind P Sn ps sh skt a :
-    let Sn' := (<[sh:=(skt <| saddress := Some a |>, ∅)]> Sn) in
-    let P' := (<[ip_of_address a:={[port_of_address a]} ∪ ps]> P) in
-    P !! ip_of_address a = Some ps →
-    bound_ports_coh Sn P →
-    bound_ports_coh Sn' P'.
-  Proof.
-    rewrite /bound_ports_coh /=.
-    intros HP HbpsCoh sh' skt' a' P' r' Hsh' Hskt' HP'.
-    destruct (decide (sh' = sh)); simplify_map_eq.
-    - rewrite lookup_insert in Hsh'; simplify_map_eq.
-      rewrite lookup_insert in HP'; by set_solver.
-    - rewrite lookup_insert_ne // in Hsh'.
-      destruct (decide ((ip_of_address a') = (ip_of_address a)))
-        as [Heq|]; simplify_map_eq.
-      + destruct Heq.
-        rewrite lookup_insert in HP'. simplify_eq /=.
-        destruct (decide (port_of_address a' = port_of_address a));
-          [set_solver|].
-        apply elem_of_union_r. by eapply HbpsCoh.
-      + rewrite lookup_insert_ne in HP'; [|done].
-        by eapply HbpsCoh.
-  Qed.
-
-(*
-  Lemma bound_ports_coh_insert_received a skt sh Sn P R T m :
-    Sn !! sh = Some (skt, R, T) →
-    saddress skt = Some a →
-    bound_ports_coh Sn P →
-    bound_ports_coh (<[sh:=(skt, {[m]} ∪ R, T)]> Sn) P.
-  Proof.
-    intros ??? sh' skt' ????.
-    destruct (decide (sh = sh')); simplify_map_eq.
-    - intros; simplify_eq; eauto.
-    - rewrite lookup_insert_ne //; eauto.
-  Qed.
-   *)
-
-  (** socket_handlers_coh *)
-  Lemma socket_handlers_coh_alloc_socket Sn sh s :
-    saddress s = None →
-    socket_handlers_coh Sn →
-    socket_handlers_coh (<[sh:=(s, ∅)]> Sn).
-  Proof.
-    intros ?? sh1 sh2 * ??? H. symmetry in H.
-    ddeq sh1 sh2; ddeq sh1 sh; ddeq sh2 sh; eauto.
-  Qed.
-
-
-  Lemma socket_handlers_coh_socketbind Sn sh skt a :
-    (∀ sh' skt' r' a',
-        Sn !! sh' = Some (skt', r') →
-        saddress skt' = Some a' →
-        port_of_address a' ≠ port_of_address a) →
-    socket_handlers_coh Sn →
-    socket_handlers_coh (<[sh:=(skt <| saddress := Some a |>, ∅)]> Sn).
-  Proof.
-    intros ? Hscoh sh1 sh2 skt1 skt2 ????? Heq.
-    ddeq sh1 sh; ddeq sh2 sh; simplify_eq=>//.
-    - destruct skt, skt2; simplify_map_eq. set_solver.
-    - destruct skt, skt1. simplify_map_eq. set_solver.
-    - destruct skt1, skt2. simplify_map_eq. eapply Hscoh; eauto.
-  Qed.
-
-  (*
-  Lemma socket_handlers_coh_insert_received Sn sh skt m R T :
-    Sn !! sh = Some (skt, R, T) →
-    socket_handlers_coh Sn →
-    socket_handlers_coh (<[sh:=(skt, {[m]} ∪ R, T)]> Sn).
-  Proof.
-    intros ?? sh1 sh2 * ??? H. symmetry in H.
-    ddeq sh1 sh2; ddeq sh1 sh; ddeq sh2 sh; eauto.
-  Qed.
-   *)
-
-  (** socket_messages_coh *)
-  Lemma socket_messages_coh_update_socket Sn sh skt :
-    socket_messages_coh Sn →
-    socket_messages_coh (<[sh:=(skt, ∅)]> Sn).
-  Proof. intros ? sh' **. ddeq sh sh'; [set_solver|]. eauto. Qed.
-
-  Lemma socket_messages_coh_insert_received a sh skt m r Sn :
-    Sn !! sh = Some (skt, r) →
-    m_destination m = a →
-    saddress skt = Some a →
-    socket_messages_coh Sn →
-    socket_messages_coh (<[sh:=(skt, {[m]} ∪ r)]> Sn).
-  Proof.
-    intros ??? Hmcoh sh' skt' r' a' Hsh' ?.
-    destruct (decide (sh = sh')); simplify_eq; last first.
-    { rewrite lookup_insert_ne // in Hsh'. by eapply Hmcoh. }
-    rewrite lookup_insert in Hsh'; simplify_eq.
-    intros m' [?%elem_of_singleton_1 | HR]%elem_of_union; subst; [done|].
-    by eapply Hmcoh.
-  Qed.
-
-  (** socket_addresses_coh *)
-  Lemma socket_addresses_coh_alloc_socket Sn sh skt n :
-    saddress skt = None →
-    socket_addresses_coh Sn n →
-    socket_addresses_coh (<[sh:=(skt, ∅)]> Sn) n.
-  Proof. intros ? ? sh' **. ddeq sh' sh; eauto. Qed.
-
-  Lemma socket_addresses_coh_socketbind Sn sh skt a :
-    saddress skt = None →
-    socket_addresses_coh Sn (ip_of_address a) →
-    socket_addresses_coh (<[sh:=(skt <| saddress := Some a |>, ∅)]> Sn) (ip_of_address a).
-  Proof. intros ? ? sh' **; ddeq sh sh'; eauto. Qed.
-
-  Lemma socket_addresses_coh_insert_received sh a skt m r Sn :
-    saddress skt = Some a →
-    socket_addresses_coh Sn (ip_of_address a) →
-    socket_addresses_coh (<[sh:=(skt, {[m]} ∪ r)]> Sn) (ip_of_address a).
-  Proof. intros ?? sh' **; ddeq sh sh'; eauto. Qed.
-
-  (** network_sockets_coh *)
-  Lemma network_sockets_coh_alloc_node Sn ps ip :
-    Sn !! ip = None →
-    network_sockets_coh Sn ps →
-    network_sockets_coh (<[ip:=∅]> Sn) ps.
-  Proof.
-    rewrite /network_sockets_coh.
-    intros ? Hcoh ip' ? Hst.
-    destruct (decide (ip' = ip)); simplify_eq.
-    - apply lookup_insert_rev in Hst. subst. split; done.
-    - eapply Hcoh; by rewrite lookup_insert_ne in Hst.
-  Qed.
-
-
-  Lemma network_sockets_coh_init n P : network_sockets_coh {[n:= ∅]} P.
-  Proof.
-    rewrite /network_sockets_coh.
-    intros n' Sn' HSn.
-    ddeq n' n;
-      [rewrite lookup_insert in HSn
-      |rewrite lookup_insert_ne in HSn];
-      rewrite /bound_ports_coh
-              /socket_handlers_coh
-              /socket_messages_coh
-              /socket_addresses_coh;
-      set_solver.
-  Qed.
-
-    Lemma network_sockets_coh_alloc_socket S Sn P n sh skt :
-    S !! n = Some Sn →
-    Sn !! sh = None →
-    saddress skt = None →
-    network_sockets_coh S P →
-    network_sockets_coh (<[n:=<[sh:=(skt, ∅)]> Sn]> S) P.
-  Proof.
-    rewrite /network_sockets_coh.
-    intros ??? Hnets n' Sn' HSn. ddeq n' n; [|eauto].
-    destruct (Hnets n Sn) as (?&?&?&?); [done|].
-    split; [by apply bound_ports_coh_alloc_socket|].
-    split; [by apply socket_handlers_coh_alloc_socket|].
-    split; [by apply socket_messages_coh_update_socket|].
-    by apply socket_addresses_coh_alloc_socket.
-  Qed.
-
-  Lemma network_sockets_coh_socketbind S P Sn ps sh skt a :
-    let ip := ip_of_address a in
-    let S' := <[ip:= <[sh:= (skt <| saddress := Some a |>, ∅)]> Sn]> S in
-    let P' := (<[ip:={[port_of_address a]} ∪ ps]> P) in
-    S !! ip = Some Sn →
-    P !! ip = Some ps →
-    Sn !! sh = Some (skt, ∅) →
-    port_of_address a ∉ ps →
-    saddress skt = None →
-    network_sockets_coh S P  →
-    network_sockets_coh S' P'.
-  Proof.
-    rewrite /network_sockets_coh /=.
-    intros ????? Hncoh ip Sn' ?.
-    assert
-      (∀ sh' skt' r' a',
-          Sn !! sh' = Some (skt', r') →
-          saddress skt' = Some a' →
-          port_of_address a' ≠ port_of_address a ).
-    { destruct (Hncoh (ip_of_address a) Sn) as
-          (HBpCoh & HshCoh & HmrCoh & HsaCoh);
-        [done|].
-      intros ** Hp.
-      assert (ip_of_address a' = ip_of_address a) as Heq.
-      { eapply HsaCoh; eauto. }
-      assert (port_of_address a' ∈ ps) as Hin.
-      { eapply HBpCoh; eauto. rewrite Heq //. }
-      rewrite Hp in Hin. set_solver. }
-    ddeq ip (ip_of_address a).
-    - destruct (Hncoh (ip_of_address a) Sn) as (?&?&?&?); [done|].
-      split; [by eapply bound_ports_coh_socketbind|].
-      split; [by eapply socket_handlers_coh_socketbind|].
-      split; [by eapply socket_messages_coh_update_socket|].
-      by eapply socket_addresses_coh_socketbind.
-    - destruct (Hncoh ip Sn') as (HBpCoh & HshCoh & HmrCoh & HsaCoh); [done|].
-      split; [|done].
-      intros ? skt' a' ???? Hps.
-      assert (ip_of_address a' = ip).
-      { eapply HsaCoh; eauto. }
-      simplify_eq /=. rewrite lookup_insert_ne in Hps; [|done].
-      by eapply HBpCoh.
-  Qed.
-
-  (*
-  Lemma network_sockets_coh_insert_sent S P M Sn sh skt a to m R T :
-    let ip := ip_of_address a in
-    let msg := mkMessage a to (sprotocol skt) m in
-    saddress skt = Some a →
-    S !! ip = Some Sn →
-    Sn !! sh = Some (skt, R, T) →
-    network_sockets_coh S M P →
-    network_sockets_coh (<[ip:=<[sh:=(skt, R, {[msg]} ∪ T)]> Sn]> S) ({[msg]} ∪ M) P.
-  Proof.
-    intros ip msg Hsa Hsi Hh HnetCoh ip' Sn' Hip'.
-    ddeq ip' ip.
-    - destruct (HnetCoh ip Sn Hsi) as (HBpCoh & HshCoh & HsmCoh & HsaCoh).
-      split.
-      { intros sh' skt' **. ddeq sh' sh; eauto using HBpCoh. }
-      split.
-      { intros sh1 sh2 skt1 skt2 ???? Hsh1 Hsh2 Hskt1 Hsaddr.
-        ddeq sh1 sh; ddeq sh2 sh; simplify_eq /=;
-          eapply HshCoh; eauto; eapply mk_is_Some; rewrite Hsaddr //. }
-      split.
-      { intros sh' **; ddeq sh' sh; split; intros;
-          edestruct HsmCoh; set_solver. }
-      intros sh' **; ddeq sh' sh; eauto.
-    - destruct (HnetCoh ip' Sn' Hip') as (HBpCoh & HshCoh & HsmCoh & HsaCoh).
-      split; eauto. split; eauto. split; last done.
-      intros sh' **. edestruct HsmCoh; eauto.
-      split; intros ??; set_solver.
-  Qed.
-
-  Lemma network_sockets_coh_not_received a skt sh S Sn P M R T m :
-    S !! ip_of_address a = Some Sn →
-    Sn !! sh = Some (skt, R, T) →
-    saddress skt = Some a →
-    m_destination m = a →
-    m ∈ M →
-    m ∉ R →
-    network_sockets_coh S M P →
-    ¬ message_received S m.
-  Proof.
-    intros HS HSn Hskt Hd HM HR Hsock Hr.
-    destruct Hr as (Sn' & sh' & skt' & a' & R' & T' & HS' & HSn' & Hs' & Hm).
-    destruct (decide (a = a')) as [ | Ha]; simplify_eq.
-    - assert (sh = sh') as <-.
-      { eapply Hsock; eauto. rewrite Hs' //. }
-      by simplify_eq.
-    - destruct (Hsock (ip_of_address a') Sn')
-        as (?&Hhandlers'&Hmsg'&?); [done|].
-      destruct (Hmsg' _ _ _ _ a' HSn') as [HR' ?]; [done|].
-      by destruct (HR' _ Hm) as [? ?].
-  Qed.
-
-  Lemma network_sockets_coh_insert_received a skt sh S Sn P M R T m :
-    let S' := (<[ip_of_address a:=<[sh:=(skt, {[m]} ∪ R, T)]> Sn]> S) in
-    S !! ip_of_address a = Some Sn →
-    Sn !! sh = Some (skt, R, T) →
-    saddress skt = Some a →
-    m_destination m = a →
-    m ∈ M →
-    m ∉ R →
-    network_sockets_coh S M P →
-    network_sockets_coh S' M P.
-  Proof.
-    rewrite /network_sockets_coh.
-    intros HS HSn ???? Hnet ip' Sn' HSn'.
-    destruct (decide (ip_of_address a = ip'));
-      simplify_map_eq; [|by eapply Hnet].
-    destruct (Hnet _ _ HS) as (?&?&?&?).
-    split; [by eapply bound_ports_coh_insert_received|].
-    split; [by eapply socket_handlers_coh_insert_received|].
-    split; [by eapply socket_messages_coh_insert_received|].
-    by eapply socket_addresses_coh_insert_received.
-  Qed.
-
-  Lemma network_sockets_messages_coh_insert_received a skt sh S Sn P M R T m :
-    let S' := (<[ip_of_address a:=<[sh:=(skt, {[m]} ∪ R, T)]> Sn]> S) in
-    S !! ip_of_address a = Some Sn →
-    Sn !! sh = Some (skt, R, T) →
-    saddress skt = Some a →
-    m_destination m = a →
-    m ∈ M →
-    m ∉ R →
-    network_sockets_coh S M P →
-    network_messages_coh S M -∗
-    network_messages_coh S' M ∗
-      ∃ φ : socket_interp Σ, m_destination m ⤇ φ ∗ ▷ φ m.
-  Proof.
-    iIntros (S' ???????) "Hmcoh".
-    rewrite /network_messages_coh big_sepS_delete //.
-    iDestruct "Hmcoh" as "[[Hm | %Hr] Hmsgs]";
-      [|exfalso; by eapply network_sockets_coh_not_received].
-    iFrame.
-    assert (message_received S' m) as Hr.
-    { by eapply message_received_receive. }
-    rewrite (big_sepS_delete _ M m) //. iFrame "%".
-    iApply big_sepS_mono; [|done].
-    iIntros (??) "[? | %Hr']"; [eauto|].
-    iRight. iPureIntro.
-    by eapply message_received_insert.
-  Qed.
-*)
-
-  (*
-  (** network_coh **)
-  Lemma network_coh_init ip ips P :
-    dom (gset ip_address) P = ips →
-    (∀ ip, ip ∈ ips → P !! ip = Some ∅) →
-    ⊢ network_sockets_coh {[ip:=∅]} ∅ P.
-  Proof.
-    intros ??. rewrite /network_coh /network_messages_coh.
-    iSplit; [|done].
-    iPureIntro. rewrite /network_sockets_coh.
-    intros ?? [<- <-]%lookup_singleton_Some.
-    rewrite /bound_ports_coh /socket_handlers_coh
-            /socket_messages_coh /socket_addresses_coh.
-    set_solver.
-  Qed.
-
-   *)
-
-  (*
-  Lemma network_coh_sent_valid m sh a skt S Sn M P R T :
-    S !! ip_of_address a = Some Sn →
-    Sn !! sh = Some (skt, R, T) →
-    saddress skt = Some a →
-    m ∈ T →
-    network_coh S M P -∗ ⌜m ∈ M⌝.
-  Proof.
-    iIntros (Hs HSn Ha Hm) "(%Hscoh & _)". iPureIntro.
-    destruct (Hscoh _ Sn Hs) as (?&?& Hmsgs &?).
-    edestruct (Hmsgs sh) as [? HT]; [done..|].
-    by apply HT.
-  Qed.
-
-  Lemma network_coh_received_valid m sh a skt S Sn M P R T :
-    S !! ip_of_address a = Some Sn →
-    Sn !! sh = Some (skt, R, T) →
-    saddress skt = Some a →
-    m ∈ R →
-    network_coh S M P -∗ ⌜m ∈ M⌝.
-  Proof.
-    iIntros (Hs HSn Ha Hm) "(%Hscoh & _)". iPureIntro.
-    destruct (Hscoh _ Sn Hs) as (?&?& Hmsgs &?).
-    edestruct (Hmsgs sh) as [HR ?]; [done..|].
-    by apply HR.
-  Qed.
-
-  Lemma network_coh_alloc_node Sn M ps ip :
-    Sn !! ip = None →
-    network_coh Sn M ps -∗
-    network_coh (<[ip:=∅]>Sn) M ps.
-  Proof.
-    iIntros (Hnone) "[% Hmsg]".
-    rewrite /network_coh.
-    iSplitR; last first.
-    { by iApply network_messages_coh_alloc_node. }
-    iPureIntro.
-    by apply network_sockets_coh_alloc_node.
-  Qed.
-
-  Lemma network_coh_alloc_socket S M P Sn n sh skt :
-    S !! n = Some Sn →
-    Sn !! sh = None →
-    saddress skt = None →
-    network_coh S M P -∗
-    network_coh (<[n:=<[sh:=(skt, ∅, ∅)]> Sn]> S) M P.
-  Proof.
-    iIntros (? ? ?) "(% & Hmsg)". iSplitR.
-    - iPureIntro. by apply network_sockets_coh_alloc_socket.
-    - by iApply network_messages_coh_alloc_socket.
-  Qed.
-
-  Lemma network_coh_socketbind S P M Sn ps sh skt a :
-    let ip := ip_of_address a in
-    S !! ip = Some Sn →
-    Sn !! sh = Some (skt, ∅, ∅) →
-    P !! ip = Some ps →
-    saddress skt = None →
-    port_of_address a ∉ ps →
-    network_coh S M P -∗
-    network_coh
-    (<[ip:=<[sh:=(skt <| saddress := Some a |>, ∅, ∅)]> Sn]> S) M
-    (<[ip:= {[port_of_address a]} ∪ ps]> P).
-  Proof.
-    iIntros (??????) "(% & Hmsg)". iSplit.
-    - iPureIntro; by apply network_sockets_coh_socketbind.
-    - by iDestruct (network_messages_coh_socketbind with "Hmsg") as "Hmsg".
-  Qed.
-
-  Lemma network_coh_insert_sent S P M Sn sh skt a to m (φ : socket_interp Σ) R T :
-    let ip := ip_of_address a in
-    let msg := mkMessage a to (sprotocol skt) m in
-    let S' := <[ip := <[sh:=(skt, R, {[msg]} ∪ T)]> Sn]> S in
-    let M' := {[msg]} ∪ M in
-    saddress skt = Some a →
-    S !! ip = Some Sn →
-    Sn !! sh = Some (skt, R, T) →
-    to ⤇ φ -∗
-    φ msg -∗
-    network_coh S M P -∗ network_coh S' M' P.
-  Proof.
-    iIntros (???????) "Hpred Hr [% Hmsg]". iSplit.
-    - iPureIntro. by apply network_sockets_coh_insert_sent.
-    - by iApply (network_messages_coh_insert_sent with "Hpred Hr Hmsg").
-  Qed.
-
-  Lemma network_coh_receive a sh skt S Sn M P R T m :
-    let ip := ip_of_address a in
-    let S' := (<[ip:=<[sh:=(skt, {[m]} ∪ R, T)]> Sn]> S) in
-    saddress skt = Some a →
-    S !! ip = Some Sn →
-    Sn !! sh = Some (skt, R, T) →
-    m_destination m = a →
-    m ∈ M →
-    m ∉ R →
-    network_coh S M P -∗ network_coh S' M P ∗ ∃ φ, m_destination m ⤇ φ ∗ ▷ φ m.
-  Proof.
-    simpl. iIntros (??????) "[%Hsock Hmcoh]".
-    rewrite /network_coh.
-    iDestruct (network_sockets_messages_coh_insert_received with "Hmcoh")
-      as "[Hmcoh Hφ]"; [done..|].
-    iFrame. iPureIntro.
-    by apply network_sockets_coh_insert_received.
-   Qed.*)
-
-  (** socket_interp_coh *)
-  Lemma socket_interp_coh_init ips A M σ f :
-    dom (gset _) M = A →
-    dom (gset _) (state_ports_in_use σ) = ips →
-    (∀ ip, ip ∈ ips → state_ports_in_use σ !! ip = Some ∅) →
-    (∀ a, a ∈ A → ip_of_address a ∈ ips) →
-    ([∗ set] a ∈ A, a ⤇ f a)%I -∗
-    fixed A -∗
-    saved_si_auth M -∗
-    socket_interp_coh (state_ports_in_use σ).
-  Proof.
-    iIntros (Hdmsi Hipdom Hpiiu Hfixdom) "? ? ?".
-    rewrite /socket_interp_coh. iExists _; iFrame.
-    iExists _; iFrame; iFrame "#".
-    rewrite -!Hdmsi.
-    iSplit; [iApply (big_sepS_mono with "[$]"); auto|].
-    iSplit; [iPureIntro; set_solver|].
-    iPureIntro. intros b Hbips. split; auto.
-    intros [Hb | [Hb HP]]; [done|].
-    simplify_eq.
-    specialize (Hpiiu _ Hbips).
-    specialize (HP _ Hpiiu). done.
-  Qed.
-
-  (*
-  Lemma socket_interp_coh_fixed_valid a A ips :
-    a ∈ A →
-    socket_interp_coh ips -∗ fixed A -∗ ∃ φ, a ⤇ φ.
-  Proof.
-    iIntros (HaA) "Hscoh #HA".
-    iDestruct "Hscoh" as (si A') "(HA' & Hsiauth & Hsis & % & H)".
-    iDestruct "H" as %Hdom.
-    iDestruct (fixed_agree with "HA HA'") as %->.
-    iDestruct (big_sepS_elem_of with "Hsis") as "$".
-    erewrite Hdom; eauto.
-  Qed.
-
-  Lemma socket_interp_coh_socketbind_static ps P a A:
-    a ∈ A →
-    P !! ip_of_address a = Some ps →
-    port_of_address a ∉ ps →
-    fixed A -∗
-    socket_interp_coh P -∗
-    socket_interp_coh (<[ip_of_address a:={[port_of_address a]} ∪ ps]> P).
-  Proof.
-    iIntros (???) "HA". rewrite /socket_interp_coh.
-    iDestruct 1 as (si A') "(HA' & Hsiauth & Hsis & %Hf & %Hdms)".
-    iDestruct (fixed_agree with "HA HA'") as %->.
-    iExists _,_. iFrame. iPureIntro. split.
-    { intros ??. rewrite dom_insert elem_of_union; right. by apply Hf. }
-    intros b. rewrite dom_insert elem_of_union. intros Hb.
-    rewrite Hdms; last first.
-    { destruct (decide (a = b)); subst; first by apply Hf.
-      destruct Hb as [->%elem_of_singleton_1|]; [|done]. by apply Hf. }
-    split; intros [|[Hnb Hdm]]; auto.
-    { right. split; [done|].
-      destruct (decide (ip_of_address a = ip_of_address b)) as [Heq|].
-      - intros P'. rewrite Heq lookup_insert. intros; simplify_eq.
-        apply elem_of_union_r, Hdm. rewrite -Heq //.
-      - intros P'. rewrite lookup_insert_ne //. apply Hdm. }
-    destruct (decide (ip_of_address a = ip_of_address b)) as [Heq|].
-    { right. split; [done|]. intros P'.
-      rewrite Heq lookup_insert in Hdm.
-      specialize (Hdm ({[port_of_address a]} ∪ _) eq_refl).
-      apply elem_of_union in Hdm. destruct Hdm as [Hdm%elem_of_singleton_1 | Hdm].
-      - destruct a, b; simpl in *. by subst.
-      - rewrite -Heq. by intros; simplify_eq. }
-    right. split; [done|].
-    rewrite lookup_insert_ne in Hdm; done.
-  Qed.
-
-  Lemma socket_interp_coh_socketbind_dynamic ps P a A φ :
-    a ∉ A →
-    P !! ip_of_address a = Some ps →
-    port_of_address a ∉ ps →
-    fixed A -∗
-    socket_interp_coh P ==∗
-    socket_interp_coh (<[ip_of_address a:={[port_of_address a]} ∪ ps]> P) ∗
-    a ⤇ φ.
-  Proof.
-    iIntros (? Hpa Hps) "#HA". rewrite /socket_interp_coh.
-    iDestruct 1 as (si A') "(HA' & Hsiauth & Hsis & %Hf & %Hdms)".
-    iDestruct (fixed_agree with "HA HA'") as %<-.
-    assert (si !! a = None).
-    { destruct (si !! a) eqn:Heq; last done.
-      destruct (Hdms a) as [[|[Hfx HP]] _]; try done.
-      - by eapply elem_of_dom_2.
-      - rewrite elem_of_dom. eauto.
-      - by apply HP in Hpa. }
-    iMod (socket_interp_alloc a φ with "Hsiauth")
-      as (?) "[Hsiauth #Hφ]"; [done|].
-    iFrame "Hφ". iModIntro. iExists _, _; iFrame.
-    iSplitL "Hsis".
-    { rewrite dom_insert_L big_sepS_insert;
-        last rewrite not_elem_of_dom //.
-      iFrame. iExists _. iFrame "Hφ". }
-    iSplit.
-    { iPureIntro. intros b Hb.
-      destruct (decide (a = b)); subst; first done.
-      apply dom_insert, elem_of_union. by auto. }
-    iPureIntro. intros b Hbdom.
-    rewrite dom_insert elem_of_union elem_of_singleton Hdms; last first.
-    { destruct (decide (ip_of_address a = ip_of_address b)) as [Heq|].
-      - destruct Heq. by eapply elem_of_dom_2.
-      - apply dom_insert, elem_of_union in Hbdom. set_solver. }
-    split.
-    - intros [Hb | Hdom]; subst.
-      + right. split; [done|]. rewrite lookup_insert.
-        intros; simplify_eq. by apply elem_of_union_l, elem_of_singleton.
-      + destruct Hdom as [? | [Hb HP]]; first by left.
-        right. split; first done.
-        destruct (decide (ip_of_address a = ip_of_address b)) as [Heq |Hneq].
-        * destruct Heq. rewrite lookup_insert. intros; simplify_eq.
-          apply elem_of_union_r, HP; eauto.
-        * by rewrite lookup_insert_ne.
-    - intros [Hb | [Hb Hdom]]; first by auto.
-      destruct (decide (a = b)) as [Heq | Hneq]; first by auto.
-      right; right. split; first done.
-      destruct (decide (ip_of_address a = ip_of_address b)) as [Heq|].
-      + intros ps'.
-        rewrite Heq in Hdom.
-        rewrite lookup_insert in Hdom.
-        specialize (Hdom ({[port_of_address a]} ∪ ps) eq_refl).
-        apply elem_of_union in Hdom. destruct Hdom as [Hdom | Hport].
-        * apply elem_of_singleton_1 in Hdom.
-          destruct a,b; simpl in *; simplify_eq.
-        * intros. destruct Heq; simplify_eq; eauto.
-      + intros. apply Hdom. rewrite lookup_insert_ne //.
-  Qed. *)
 
   (** aneris_state_interp *)
   Lemma mapsto_node_heap_valid n γs σ :
@@ -1402,7 +52,6 @@ Section state_interpretation.
     iApply (mapsto_node_heap_valid with "[$] [$]").
   Qed.
 
-
   Lemma mapsto_node_valid_sockets n γs σ :
     aneris_state_interp σ -∗
     mapsto_node n γs -∗
@@ -1424,83 +73,24 @@ Section state_interpretation.
     iApply (mapsto_node_valid_sockets with "[$] [$]").
   Qed.
 
-  (** get_message_history *)
-  Lemma get_message_history_empty ip a :
-    get_address_messages {[ip := ∅]} a = (∅, ∅).
+   Lemma messages_ctx_alloc_node ip ports mhγ:
+    mhγ !! ip = None →
+    messages_ctx mhγ ==∗
+                 messages_ctx (<[ip := messages_init ports ]>mhγ) ∗
+                 ([∗ set] p ∈ ports, SocketAddressInet ip p ⤳ (∅, ∅)).
   Proof.
-    rewrite /get_address_messages.
-    ddeq ip (ip_of_address a); by simplify_map_eq /=.
-  Qed.
-
-  (** messages_history_coh *)
-  Lemma messages_history_coh_init ip :
-    messages_history_coh ∅ {[ip := ∅]} {[ip := ∅]}.
-  Proof.
-    rewrite /messages_history_coh
-            /message_soup_coh /receive_buffers_coh /messages_addresses_coh.
-    split; first set_solver.
-    split; first by intros; simplify_map_eq.
-    intros ? ? ? Hgam.
-    split; rewrite get_message_history_empty in Hgam; set_solver.
-  Qed.
-
-  (** messages_sent *)
-  Lemma messages_sent_empty ip : messages_sent {[ip:=∅]} = ∅.
-  Proof.
-    rewrite -insert_empty.
-    rewrite -insert_delete.
-    rewrite /messages_sent map_fold_insert_L; [set_solver | | set_solver].
-    intros j j' z z' m Hneq Hj Hj'.
-    assert (z = ∅) as ->.
-    { rewrite insert_delete insert_empty in Hj Hj'.
-      ddeq j ip.
-      - rewrite lookup_insert in Hj. set_solver.
-      - rewrite lookup_insert_ne in Hj; set_solver. }
-    assert (z' = ∅) as ->.
-     { rewrite insert_delete insert_empty in Hj Hj'.
-      ddeq j' ip.
-      - rewrite lookup_insert in Hj'. set_solver.
-      - rewrite lookup_insert_ne in Hj'; set_solver. }
-    done.
-  Qed.
-
-  Lemma messages_resource_coh_init ip : ⊢ messages_resource_coh {[ip := ∅]}.
-  Proof.
-    iIntros. by rewrite /messages_resource_coh messages_sent_empty.
-  Qed.
-
-  Lemma config_wp_correct `{anerisG Σ} : ⊢ config_wp.
-  Proof.
-    rewrite /config_wp.
-    iIntros.
-    iModIntro.
-    iIntros (σ1 k σ2 ks nt Hstep) "Hst".
-    rewrite /state_interp; simplify_eq /=.
-    iDestruct "Hst"
-      as (m mhγ)
-           "(%Hgcoh & %Hnscoh & %Hmhcoh
-                    & Hnauth & Hsi & Hlcoh & Hfreeips & Hmctx & Hmres)".
-    iApply step_fupd_fupd; iApply step_fupd_intro; first done.
-    iExists m, mhγ.
-    iFrame.
-    iIntros "!> !>".
-    (* TODO: The only subtle point will be to show that receive_buffers_coh is
-     preserved for delivery config step. *)
+  (*   revert σ;
+       induction σ' as [| l v σ' Hl IH] using map_ind; iIntros (σ Hdisj) "Hσ".
+    { rewrite left_id_L. auto. }
+    iMod (IH with "Hσ") as "[Hσ'σ Hσ']"; first by eapply map_disjoint_insert_l.
+    decompose_map_disjoint.
+    rewrite !big_opM_insert // -insert_union_l //.
+    by iMod (gen_heap_light_alloc with "Hσ'σ") as "($ & $ & $)";
+      first by apply lookup_union_None.
+  Qed. *)
   Admitted.
 
-  (* receive_buffers_coh *)
-  Lemma receive_buffers_coh_alloc_socket σ mhγ s sh ip Sn :
-    state_sockets σ !! ip = Some Sn →
-    Sn !! sh = None →
-    receive_buffers_coh (state_sockets σ) mhγ →
-    receive_buffers_coh (<[ip:=<[sh:=(s, ∅)]> Sn]> (state_sockets σ)) mhγ.
-  Proof.
-    rewrite /receive_buffers_coh.
-    intros HSn HNone Hrbcoh ip' Sn' sh' skt' r' m' HSn' Hskt' Hm'.
-    ddeq ip ip'.
-    - ddeq sh sh'; [ done | by eapply Hrbcoh ].
-    - by eapply Hrbcoh.
-  Qed.
+
 
     (* aneris_state_interp *)
   Lemma aneris_state_interp_init ips A σ f M ip γs :
@@ -1577,22 +167,6 @@ Section state_interpretation.
       by iApply free_ips_coh_free_ports_valid.
   Qed.
 
-  Lemma messages_ctx_alloc_node ip ports mhγ:
-    mhγ !! ip = None →
-    messages_ctx mhγ ==∗
-                 messages_ctx (<[ip := messages_init ports ]>mhγ) ∗
-                 ([∗ set] p ∈ ports, SocketAddressInet ip p ⤳ (∅, ∅)).
-  Proof.
-  (*   revert σ;
-       induction σ' as [| l v σ' Hl IH] using map_ind; iIntros (σ Hdisj) "Hσ".
-    { rewrite left_id_L. auto. }
-    iMod (IH with "Hσ") as "[Hσ'σ Hσ']"; first by eapply map_disjoint_insert_l.
-    decompose_map_disjoint.
-    rewrite !big_opM_insert // -insert_union_l //.
-    by iMod (gen_heap_light_alloc with "Hσ'σ") as "($ & $ & $)";
-      first by apply lookup_union_None.
-  Qed. *)
-  Admitted.
 
   Lemma aneris_state_interp_alloc_node σ ip ports :
     aneris_state_interp σ ∗ free_ip ip ==∗
@@ -1731,7 +305,10 @@ Section state_interpretation.
   Lemma aneris_state_interp_socket_valid σ sh ip q skt:
     aneris_state_interp σ -∗
     sh ↪[ip]{q} skt -∗
-    ∃ Sn r, ⌜state_sockets σ !! ip = Some Sn ∧ Sn !! sh = Some (skt, r)⌝.
+    ∃ Sn r,
+      ⌜state_sockets σ !! ip = Some Sn ∧
+      Sn !! sh = Some (skt, r) ∧
+      (saddress skt = None → r = ∅)⌝.
   Proof.
     iIntros "Hσ Hsh".
     iDestruct "Hσ"
@@ -1741,11 +318,17 @@ Section state_interpretation.
     rewrite mapsto_socket_eq.
     iDestruct "Hsh" as (γs' r) "[#Hip Hsh]".
     iDestruct (node_gnames_valid with "Hnauth Hip") as "%Hmin".
-    iApply (local_state_coh_valid_sockets  _ _ γs' _ q with "[Hlcoh] [Hsh]").
+    iPoseProof (local_state_coh_valid_sockets  _ _ γs' _ q with "[Hlcoh] [Hsh]")
+      as (Sn r0 ) "(%Hp1 & %Hp2)".
     - iDestruct (big_sepM_lookup with "Hlcoh") as "Hl"; done.
     - rewrite mapsto_socket_eq.
       unfold mapsto_socket_def.
       eauto with iFrame.
+    - iExists Sn, r0.
+      iPureIntro.
+      repeat split; try done.
+      specialize (Hnscoh ip Sn Hp1) as (?&?&?&?&Hb).
+      by eapply Hb.
   Qed.
 
   Lemma aneris_state_interp_alloc_socket s ip sh Sn σ :
@@ -1791,63 +374,91 @@ Section state_interpretation.
   Qed.
 
 
-  (*
-  Lemma aneris_state_interp_socketbind_static σ1 a sh skt ps Sn A :
+  Lemma mapsto_socket_mapsto_node h s ip :
+    h ↪[ip] s ⊢ h ↪[ip] s ∗ ∃ γs, mapsto_node ip γs.
+  Proof.
+    rewrite mapsto_socket_eq /mapsto_socket_def.
+    iDestruct 1 as (γs' r) "[#Hn Hsh]".
+    iSplitL; eauto with iFrame.
+  Qed.
+
+  Lemma aneris_state_interp_socketbind_static σ1 a sh skt ps Sn A r :
     let ip := ip_of_address a in
-    let S' := <[ip := <[sh:=(skt<| saddress := Some a |>, ∅, ∅)]> Sn]> (state_sockets σ1) in
+    let S' :=
+        <[ip := <[sh:=(skt<| saddress := Some a |>, r)]> Sn]>
+        (state_sockets σ1) in
     let P' := <[ip := {[port_of_address a]} ∪ ps]> (state_ports_in_use σ1) in
     let σ2 := σ1 <| state_sockets := S' |> <| state_ports_in_use := P' |> in
     state_sockets σ1 !! ip = Some Sn →
-    Sn !! sh = Some (skt, ∅, ∅) →
+    Sn !! sh = Some (skt, r) →
     state_ports_in_use σ1 !! ip = Some ps →
     saddress skt = None →
     a ∈ A →
     aneris_state_interp σ1 -∗
     fixed A -∗
-    sh ↪[ip_of_address a] (skt, ∅, ∅) -∗
+    sh ↪[ip_of_address a] skt -∗
     free_ports ip {[port_of_address a]} ==∗
-    aneris_state_interp σ2 ∗ sh ↪[ip] (skt<| saddress := Some a |>, ∅, ∅) ∗
+    aneris_state_interp σ2 ∗ sh ↪[ip] (skt<| saddress := Some a |>) ∗
     ∃ φ, a ⤇ φ.
   Proof.
     simpl. iIntros (?????) "Hσ #HA Hsh Hp".
-    iDestruct "Hσ" as (m) "(Hnauth & % & Hsock & Hlcoh & Hfreeips & Hnet)".
-    iDestruct "Hsh" as (?) "[#Hn Hsh]".
+    iDestruct "Hσ"
+      as (m mhγ)
+           "(%Hgcoh & %Hnscoh & %Hmhcoh
+                    & Hnauth & Hsi & Hlcoh & Hfreeips & Hmctx & Hmres)".
+    iDestruct (mapsto_socket_mapsto_node with "Hsh") as "(Hsh & #Hn)".
+    iDestruct "Hn" as (γs) "Hn".
     iDestruct (node_gnames_valid with "Hnauth Hn") as %?.
     iDestruct (big_sepM_local_state_coh_delete with "Hlcoh")
       as "(Hstate & Hlcoh)"; [done|].
-    iMod (local_state_coh_socketbind with "[$Hstate Hsh]") as "[Hstate' $]"; try done.
-    { iExists _; eauto. }
-    iDestruct (big_sepM_local_state_coh_update_socket_notin with "Hlcoh") as "Hlcoh".
+    iMod (local_state_coh_socketbind with "[$Hstate Hsh]") as
+        "[Hstate' $]"; try done.
+    iDestruct
+      (big_sepM_local_state_coh_update_socket_notin with "Hlcoh")
+      as "Hlcoh".
     { apply lookup_delete. }
-    iDestruct (big_sepM_local_state_coh_insert with "Hstate' Hlcoh") as "Hlcoh"; [done|].
-    iDestruct (free_ips_coh_free_ports_valid with "Hfreeips Hp") as (?) "[% %]".
-    iDestruct (socket_interp_coh_fixed_valid with "Hsock HA") as "#$"; [done|].
-    simplify_eq.
-    iMod (free_ips_coh_dealloc with "Hfreeips Hp") as "Hfreeips"; [done..|].
-    iModIntro. iExists _. iFrame. rewrite /set /=.
+    iDestruct (big_sepM_local_state_coh_insert with "Hstate' Hlcoh")
+      as "Hlcoh"; [done|].
+    iDestruct (free_ips_coh_free_ports_valid with "Hfreeips Hp")
+      as (?) "[% %]".
+    iDestruct (socket_interp_coh_fixed_valid with "Hsi HA") as "#$"; [done|].
+    iMod (free_ips_coh_dealloc _ _ sh skt with "Hfreeips Hp")
+      as "Hfreeips"; [done..|].
+    iModIntro. iExists m, mhγ. iFrame. rewrite /set /=.
     iSplit.
     { iPureIntro; by eapply gnames_coh_update_sockets. }
-    iSplitL "Hsock".
-    { by iApply socket_interp_coh_socketbind_static. }
-    by iApply network_coh_socketbind.
-  Qed.
+    iSplitR.
+    { iPureIntro. admit. }
+    iSplitR.
+    { iPureIntro. admit. }
+    iSplitL "Hsi".
+    {  iApply socket_interp_coh_socketbind_static; eauto with set_solver. }
+    iFrame.
+    admit.
+      (* by iApply network_coh_socketbind. *)
+  Admitted.
 
-  Lemma aneris_state_interp_socketbind_dynamic σ1 a sh skt ps Sn A φ :
+  Lemma aneris_state_interp_socketbind_dynamic σ1 a sh skt ps Sn A φ r:
     let ip := ip_of_address a in
-    let S' := <[ip := <[sh:=(skt<| saddress := Some a |>, ∅, ∅)]> Sn]> (state_sockets σ1) in
+    let S' :=
+        <[ip := <[sh:=(skt<| saddress := Some a |>, r)]> Sn]>
+        (state_sockets σ1) in
     let P' := <[ip := {[port_of_address a]} ∪ ps]> (state_ports_in_use σ1) in
     let σ2 := σ1 <| state_sockets := S' |> <| state_ports_in_use := P' |> in
     state_sockets σ1 !! ip = Some Sn →
-    Sn !! sh = Some (skt, ∅, ∅) →
+    Sn !! sh = Some (skt, r) →
     state_ports_in_use σ1 !! ip = Some ps →
     saddress skt = None →
     a ∉ A →
     aneris_state_interp σ1 -∗
     fixed A -∗
-    sh ↪[ip_of_address a] (skt, ∅, ∅) -∗
+    sh ↪[ip_of_address a] skt -∗
     free_ports ip {[port_of_address a]} ==∗
-    aneris_state_interp σ2 ∗ sh ↪[ip] (skt<| saddress := Some a |>, ∅, ∅) ∗
+    aneris_state_interp σ2 ∗ sh ↪[ip] (skt<| saddress := Some a |>) ∗
     a ⤇ φ.
+  Proof.
+  Admitted.
+ (*
   Proof.
     simpl. iIntros (?????) "Hσ #HA Hsh Hp".
     iDestruct "Hσ" as (m) "(Hnauth & % & Hsock & Hlcoh & Hfreeips & Hnet)".
@@ -1870,7 +481,9 @@ Section state_interpretation.
     { iPureIntro; by eapply gnames_coh_update_sockets. }
     by iApply network_coh_socketbind.
   Qed.
+  *)
 
+(*
   Lemma aneris_state_interp_send sh a skt Sn R T φ to mbody σ1 :
     let ip := ip_of_address a in
     let msg := mkMessage a to (sprotocol skt) mbody in
@@ -1984,3 +597,13 @@ Section state_interpretation.
 End state_interpretation.
 
 Global Opaque aneris_state_interp.
+
+
+  (*Definition gset_ipofsa := gset_map ip_of_address.
+
+  Definition messages_history_new_node ip ps mhγ :=
+   set_fold (fun p acc => <[(SocketAddressInet ip p):=(∅, ∅)]> acc) mhγ ps.*)
+
+
+  (* Definition get_message_history mhγ sa := *)
+  (*   pms ← (mhγ !! (ip_of_address sa)); pms !! (port_of_address sa). *)
