theories/aneris_lang/state_interp_config_wp.v
@@ -1,0 +1,65 @@
+From stdpp Require Import fin_maps gmap.
+From iris.bi.lib Require Import fractional.
+From iris.proofmode Require Import tactics.
+From iris.base_logic.lib Require Import viewshifts saved_prop gen_heap.
+From iris_string_ident Require Import ltac2_string_ident.
+From aneris.program_logic Require Export weakestpre adequacy.
+From aneris.program_logic Require Import ectx_lifting.
+From aneris.program_logic Require Export gen_heap_light.
+From aneris.aneris_lang Require Export
+     aneris_lang notation network resources
+     state_interp_def
+     state_interp_local_coh
+     state_interp_gnames_coh
+     state_interp_free_ips_coh
+     state_interp_network_sockets_coh
+     state_interp_socket_interp_coh
+     state_interp_messages_resource_coh
+     state_interp_messages_history_coh.
+
+From aneris.aneris_lang.lib Require Import util.
+
+From RecordUpdate Require Import RecordSet.
+Set Default Proof Using "Type".
+
+Import uPred.
+Import Network.
+Import RecordSetNotations.
+
+Section state_interpretation.
+  Context `{!anerisG Σ}.
+
+  Lemma config_wp_correct : ⊢ config_wp.
+  Proof.
+    rewrite /config_wp.
+    iIntros.
+    iModIntro.
+    iIntros (σ1 k σ2 ks nt Hstep) "Hst".
+    rewrite /state_interp; simplify_eq /=.
+    iDestruct "Hst"
+      as (γm mhγ)
+           "(%Hgcoh & %Hnscoh & %Hmhcoh
+                    & Hnauth & Hsi & Hlcoh & Hfreeips & Hmctx & Hmres)".
+    iApply step_fupd_fupd; iApply step_fupd_intro; first done.
+    iExists γm, mhγ.
+    iFrame.
+    iIntros "!> !>".
+    destruct Hstep as
+        [ ip σ k Sn Sn' sh a skt R m Hm HSn Hsh HSn' Hsaddr | σ]; simpl.
+    { iFrame "Hsi".
+      iSplitR; [eauto using gnames_coh_deliver_message|].
+      iSplitR; [eauto using network_sockets_coh_deliver_message|].
+      iSplitR; [eauto using messages_history_coh_deliver_message|].
+      iSplitL "Hlcoh".
+      - by iApply (local_state_coh_deliver_message with "[Hlcoh]").
+      - by iApply free_ips_coh_deliver_message. }
+    iFrame.
+    iSplitR; first done.
+    iSplitR; first done.
+    iPureIntro. by eapply messages_history_drop_message.
+  Qed.
+  (* TODO: The only subtle point will be to show that receive_buffers_coh is
+     preserved for delivery config step. *)
+
+
+End state_interpretation.
