theories/aneris_lang/state_interp_def.v
@@ -1,0 +1,263 @@
+From stdpp Require Import fin_maps gmap.
+From iris.bi.lib Require Import fractional.
+From iris.proofmode Require Import tactics.
+From iris.base_logic.lib Require Import viewshifts saved_prop gen_heap.
+From iris_string_ident Require Import ltac2_string_ident.
+From aneris.program_logic Require Export weakestpre adequacy.
+From aneris.program_logic Require Import ectx_lifting.
+From aneris.program_logic Require Export gen_heap_light.
+From aneris.aneris_lang Require Export aneris_lang notation network resources.
+From aneris.aneris_lang.lib Require Import util.
+
+From RecordUpdate Require Import RecordSet.
+Set Default Proof Using "Type".
+
+Import uPred.
+Import Network.
+Import RecordSetNotations.
+
+Section definitions.
+  Context `{anerisG Σ}.
+  Implicit Types σ : state.
+  Implicit Types h : heap.
+  Implicit Types H : gmap ip_address heap.
+  Implicit Types S : gmap ip_address sockets.
+  Implicit Types Sn : sockets.
+  Implicit Types P : ports_in_use.
+  Implicit Types ps : gset port.
+  Implicit Types ips : gset ip_address.
+  Implicit Types M R T : message_soup.
+  Implicit Types m : message.
+  Implicit Types a : socket_address.
+  Implicit Types ip : ip_address.
+  Implicit Types sh : socket_handle.
+  Implicit Types skt : socket.
+  Implicit Types A B : gset socket_address.
+  Implicit Types pms : gmap port (message_soup * message_soup).
+  Implicit Types mhγ : gmap ip_address (gmap port (message_soup * message_soup)).
+  Implicit Types γm : gmap ip_address node_gnames.
+  Implicit Types sis : gmap socket_address gname.
+
+  (** Definitions for the message history *)
+
+  (* The set of all received messages *)
+  Definition messages_received mhγ :=
+    map_fold (fun ip pms acc0 =>
+                map_fold (fun p rt acc1 => rt.1 ∪ acc1) acc0 pms) ∅ mhγ.
+  (* The set of all transmitted messages *)
+  Definition messages_sent mhγ :=
+    map_fold (fun ip pms acc0 =>
+                map_fold (fun p rt acc1 => rt.2 ∪ acc1) acc0 pms) ∅ mhγ.
+
+  (* [m] has been received *)
+  Definition message_received m mhγ := m ∈ (messages_received mhγ).
+
+  (* Initialization of message history from a given set of ports *)
+  Definition messages_init (ports : gset port) :=
+    set_fold (fun p macc => <[p := (∅, ∅)]>macc)
+             (∅: gmap port (message_soup * message_soup)) ports.
+
+  Definition get_address_messages mhγ sa :=
+    match (mhγ !! (ip_of_address sa)) with
+    | None => (∅, ∅)
+    | Some mps =>
+      match mps !! (port_of_address sa) with
+      | None => (∅, ∅)
+      | Some (R,T) => (R,T)
+      end
+    end.
+
+  (** Local state coherence *)
+
+  (* The local state of the node at [ip] is coherent
+     with physical state [σ] and ghost names [γs]. *)
+  Definition local_state_coh σ ip γs :=
+    (∃ h Sn,
+        ⌜state_heaps σ !! ip = Some h⌝ ∗
+        ⌜state_sockets σ !! ip = Some Sn⌝ ∗
+        mapsto_node ip γs ∗
+        heap_ctx γs h ∗
+        sockets_ctx γs Sn)%I.
+
+  (** The domains of heaps and sockets coincide with the gname map [γm] *)
+  Definition gnames_coh γm H S mhγ :=
+    dom (gset ip_address) γm = dom (gset ip_address) H ∧
+    dom (gset ip_address) γm = dom (gset ip_address) S ∧
+    dom (gset ip_address) γm = dom (gset ip_address) mhγ.
+
+  (** Socket interpretation coherence *)
+  (* Addresses with socket interpretations are bound *)
+  Definition socket_interp_coh P :=
+    (∃ sis A,
+        (* [A] is the set of addresses with fixed interpretations *)
+        fixed A ∗
+        (* [si] is the map from addresses to name of
+           saved socket interpretations *)
+        saved_si_auth sis ∗
+        (* there exists a socket interpretation for all addresses in this map *)
+        ([∗ set] s ∈ (dom (gset socket_address) sis), ∃ φ, s ⤇ φ) ∗
+        (* the addresses in A are in the domain of P *)
+        ⌜∀ a, a ∈ A → ip_of_address a ∈ dom (gset ip_address) P⌝ ∗
+        (* all addresses in [si] either have a fixed interpretation ([a ∈ A]) or
+           are dynamically bound. *)
+        ⌜∀ a, (ip_of_address a ∈ dom (gset ip_address) P) →
+              (a ∈ dom (gset socket_address) sis ↔
+                 a ∈ A ∨ (a ∉ A ∧ ∀ ps, P !! ip_of_address a = Some ps →
+                                        port_of_address a ∈ ps))⌝)%I.
+
+  (** Free ips coherence *)
+  (* Free ips have no bound ports, no heap, and no sockets  *)
+  Definition free_ips_coh σ :=
+    (∃ free_ips free_ports,
+        (* the domains of [free_ips] and [free_ports] are disjoint *)
+        (⌜dom (gset _) free_ports ## free_ips ∧
+         (* if the ip [ip] is free, no ports have been bound  *)
+         (∀ ip, ip ∈ free_ips → state_ports_in_use σ !! ip = Some ∅) ∧
+         (* if the ip [ip] is free, neither a heap nor a socket map has been
+            allocated *)
+         (∀ ip, ip ∈ free_ips →
+                state_heaps σ !! ip = None ∧ state_sockets σ !! ip = None) ∧
+         (* free ports and bound ports are disjoint *)
+         (∀ ip ps, free_ports !! ip = Some (GSet ps) →
+             ∃ bound_ports,
+               (state_ports_in_use σ) !! ip = Some bound_ports ∧
+               ps ## bound_ports )⌝) ∗
+         (* we have the auth parts of the resources for free ips and ports *)
+         free_ips_auth free_ips ∗
+         free_ports_auth free_ports)%I.
+
+  (** Network sockets coherence for bound ports, socket handlers,
+      receive buffers, and socket addresses *)
+  (* The ports of all bound addresses in [Sn] are also in [P] *)
+  Definition bound_ports_coh Sn P :=
+    ∀ sh skt a ps r,
+      Sn !! sh = Some (skt, r) →
+      saddress skt = Some a →
+      P !! ip_of_address a = Some ps →
+      (port_of_address a) ∈ ps.
+
+  (* All sockets in [Sn] with the same address have the same handler *)
+  Definition socket_handlers_coh Sn :=
+    ∀ sh sh' skt skt' r r',
+      Sn !! sh = Some (skt, r) →
+      Sn !! sh' = Some (skt', r') →
+      is_Some (saddress skt) →
+      saddress skt = saddress skt' →
+      sh = sh'.
+
+  (* Sent and received messages at all socket in [Sn] are in [M] *)
+  Definition socket_messages_coh Sn :=
+    ∀ sh skt r a,
+      Sn !! sh = Some (skt, r) →
+      saddress skt = Some a →
+      ∀ m, m ∈ r → m_destination m = a.
+
+  (* All sockets in [Sn] are bound to ip address [ip] *)
+  Definition socket_addresses_coh Sn ip :=
+    ∀ sh skt r a,
+      Sn !! sh = Some (skt, r) →
+      saddress skt = Some a →
+      ip_of_address a = ip.
+
+  (* Receive buffers of unbound sockets are empty. *)
+  Definition socket_unbound_empty_buf_coh Sn ip :=
+    ∀ sh skt r a,
+      Sn !! sh = Some (skt, r) →
+      saddress skt = None →
+      r = ∅.
+
+  Definition network_sockets_coh S P :=
+    ∀ ip Sn,
+      S !! ip = Some Sn →
+      bound_ports_coh Sn P ∧
+      socket_handlers_coh Sn ∧
+      socket_messages_coh Sn ∧
+      socket_addresses_coh Sn ip ∧
+      socket_unbound_empty_buf_coh Sn ip.
+
+  (** Message history map coherence *)
+  (* Every message present in the message soup has been
+     recorded in the logic as sent from the node of its origin. *)
+  Definition message_soup_coh M mhγ :=
+    ∀ m, m ∈ M →
+         ∃ R T, get_address_messages mhγ (m_sender m) = (R, T) ∧ m ∈ T.
+
+  (* Every message in the receive buffer has been recorded in
+     the logic as sent from the node of its origin. *)
+  Definition receive_buffers_coh S mhγ :=
+    ∀ ip Sn sh skt r m,
+      S !! ip = Some Sn →
+      Sn !! sh = Some (skt, r) →
+      m ∈ r →
+      ∃ R T, get_address_messages mhγ (m_sender m) = (R, T) ∧ m ∈ T.
+
+  (* The messages in the logical map mhγ, that tracks
+     received and transmitted messages, have coherent addresses. *)
+  Definition messages_addresses_coh mhγ :=
+    ∀ a R T, get_address_messages mhγ a = (R, T) →
+             (∀ m, m ∈ R → m_destination m = a) ∧
+             (∀ m, m ∈ T → m_sender m = a).
+
+  (* Message history is coherent w.r.t. message soup, socket map, and itself. *)
+  Definition messages_history_coh M S mhγ :=
+    message_soup_coh M mhγ ∧
+    receive_buffers_coh S mhγ ∧
+    messages_addresses_coh mhγ.
+
+ (* For all messages [m] in [M], either the network owns the resources [Φ m]
+     described by some socket protocol [Φ] or it has been delivered. *)
+  Definition messages_resource_coh mhγ :=
+    ([∗ set] m ∈ messages_sent mhγ,
+     (* either [m] is governed by a protocol and
+        the network owns the resources *)
+     (∃ (Φ : socket_interp Σ), (m_destination m) ⤇ Φ ∗ ▷ Φ m) ∨
+     (* or [m] has been delivered somewhere *)
+     ⌜message_received m mhγ⌝)%I.
+
+  (** State interpretation *)
+  Definition aneris_state_interp σ :=
+    (∃ γm mhγ,
+        ⌜gnames_coh γm (state_heaps σ) (state_sockets σ) mhγ⌝ ∗
+        ⌜network_sockets_coh (state_sockets σ) (state_ports_in_use σ)⌝ ∗
+        ⌜messages_history_coh (state_ms σ) (state_sockets σ) mhγ⌝ ∗
+        node_gnames_auth γm ∗
+        socket_interp_coh (state_ports_in_use σ) ∗
+        ([∗ map] ip ↦ γs ∈ γm, local_state_coh σ ip γs) ∗
+        free_ips_coh σ ∗
+        messages_ctx mhγ ∗
+        messages_resource_coh mhγ)%I.
+
+End definitions.
+
+
+Global Instance anerisG_irisG `{!anerisG Σ} : irisG aneris_lang Σ := {
+  iris_invG := _;
+  state_interp σ κ _ := aneris_state_interp σ;
+  fork_post _ := True%I;
+}.
+
+Global Opaque iris_invG.
+
+Local Hint Extern 0 (head_reducible _ _) => eexists _, _, _; simpl : core.
+Local Hint Constructors head_step : core.
+Local Hint Resolve alloc_fresh : core.
+Local Hint Resolve to_of_val : core.
+
+(* TODO: come up with something more reliable *)
+Ltac ddeq k1 k2 :=
+  destruct (decide (k1 = k2)); subst;
+  repeat
+    match goal with
+    | Hyp : context[ (<[_:=_]>_) !! _ ] |- _ =>
+      rewrite lookup_insert in
+          Hyp || (rewrite lookup_insert_ne in Hyp; last done);
+      simplify_eq /=
+    | Hyp : is_Some _ |- _ => destruct Hyp
+    | |- context[ (<[_:=_]>_) !! _ ] =>
+      rewrite lookup_insert || (rewrite lookup_insert_ne; last done);
+      simplify_eq /=
+    |  H1 : ?x = ?z, Heq : ?x = ?y |- _ =>
+       rewrite Heq in H1; simplify_eq /=; try eauto
+    | Hdel : context[ delete ?n ?m !! ?n = _] |- _ =>
+      rewrite lookup_delete in Hdel; simplify_eq /=
+    end.
