theories/aneris_lang/state_interp_gnames_coh.v
@@ -1,0 +1,74 @@
+From stdpp Require Import fin_maps gmap.
+From iris.bi.lib Require Import fractional.
+From iris.proofmode Require Import tactics.
+From iris.base_logic.lib Require Import viewshifts saved_prop gen_heap.
+From iris_string_ident Require Import ltac2_string_ident.
+From aneris.program_logic Require Export weakestpre adequacy.
+From aneris.program_logic Require Import ectx_lifting.
+From aneris.program_logic Require Export gen_heap_light.
+From aneris.aneris_lang Require Export
+     aneris_lang notation network resources
+     state_interp_def.
+From aneris.aneris_lang.lib Require Import util.
+
+From RecordUpdate Require Import RecordSet.
+Set Default Proof Using "Type".
+
+Import uPred.
+Import Network.
+Import RecordSetNotations.
+
+Section state_interpretation.
+  Context `{!anerisG Σ}.
+
+  (** gnames_coh *)
+  (* TODO: check whether this works out. *)
+  Lemma gnames_coh_singleton_empty ip γs :
+    gnames_coh {[ip:=γs]} {[ip:=∅]} {[ip:=∅]} {[ip:=∅]}.
+  Proof. rewrite /gnames_coh !dom_singleton_L //. Qed.
+
+  Lemma gnames_coh_singleton ip γs h Sn p R T:
+    gnames_coh {[ip:=γs]} {[ip:=h]} {[ip:=Sn]} {[ip:= {[p:=(R,T)]} ]}.
+  Proof. rewrite /gnames_coh !dom_singleton_L //. Qed.
+
+  Lemma gnames_coh_valid γm H S ip Mγ :
+    H !! ip = None →
+    gnames_coh γm H S Mγ →
+    γm !! ip = None.
+  Proof. rewrite -!not_elem_of_dom => _ [-> _] //. Qed.
+
+  Lemma gnames_coh_alloc_node γm H S ip γn mhγ ports:
+    gnames_coh γm H S mhγ →
+    gnames_coh (<[ip:=γn]> γm) (<[ip:=∅]> H) (<[ip:=∅]> S)
+               (<[ip:= messages_init ports]> mhγ).
+  Proof. rewrite /gnames_coh !dom_insert_L.
+         move=> [->] //=. set_solver.
+  Qed.
+
+  Lemma gnames_coh_update_heap n γm H S h h' Mγ:
+    H !! n = Some h →
+    gnames_coh γm H S Mγ →
+    gnames_coh γm (<[n:=h']> H) S Mγ.
+  Proof.
+    intros ?%elem_of_dom_2 [? ?].
+    rewrite /gnames_coh dom_insert_L subseteq_union_1_L //=.
+    set_solver.
+  Qed.
+
+  Lemma gnames_coh_update_sockets n γm H S Sn Sn' Mγ :
+    S !! n = Some Sn →
+    gnames_coh γm H S Mγ →
+    gnames_coh γm H (<[n:=Sn']> S) Mγ.
+  Proof.
+    intros ?%elem_of_dom_2 [? ?].
+    rewrite /gnames_coh dom_insert_L subseteq_union_1_L //=.
+    set_solver.
+  Qed.
+
+  Lemma gnames_coh_deliver_message γm mhγ H S Sn Sn' ip:
+    S !! ip = Some Sn →
+    gnames_coh γm H S mhγ →
+    gnames_coh γm H (<[ip:=Sn']> S) mhγ.
+  Proof. Admitted.
+
+End state_interpretation.
