theories/aneris_lang/state_interp_messages_history_coh.v
@@ -1,0 +1,75 @@
+From stdpp Require Import fin_maps gmap.
+From iris.bi.lib Require Import fractional.
+From iris.proofmode Require Import tactics.
+From iris.base_logic.lib Require Import viewshifts saved_prop gen_heap.
+From iris_string_ident Require Import ltac2_string_ident.
+From aneris.program_logic Require Export weakestpre adequacy.
+From aneris.program_logic Require Import ectx_lifting.
+From aneris.program_logic Require Export gen_heap_light.
+From aneris.aneris_lang Require Export
+     aneris_lang notation network resources
+     state_interp_def.
+
+From aneris.aneris_lang.lib Require Import util.
+
+From RecordUpdate Require Import RecordSet.
+Set Default Proof Using "Type".
+
+Import uPred.
+Import Network.
+Import RecordSetNotations.
+
+Section state_interpretation.
+  Context `{!anerisG Σ}.
+
+   (* receive_buffers_coh *)
+  Lemma receive_buffers_coh_alloc_socket σ mhγ s sh ip Sn :
+    state_sockets σ !! ip = Some Sn →
+    Sn !! sh = None →
+    receive_buffers_coh (state_sockets σ) mhγ →
+    receive_buffers_coh (<[ip:=<[sh:=(s, ∅)]> Sn]> (state_sockets σ)) mhγ.
+  Proof.
+    rewrite /receive_buffers_coh.
+    intros HSn HNone Hrbcoh ip' Sn' sh' skt' r' m' HSn' Hskt' Hm'.
+    ddeq ip ip'.
+    - ddeq sh sh'; [ done | by eapply Hrbcoh ].
+    - by eapply Hrbcoh.
+  Qed.
+
+  (** get_message_history *)
+  Lemma get_message_history_empty ip a :
+    get_address_messages {[ip := ∅]} a = (∅, ∅).
+  Proof.
+    rewrite /get_address_messages.
+    ddeq ip (ip_of_address a); by simplify_map_eq /=.
+  Qed.
+
+  (** messages_history_coh *)
+  Lemma messages_history_coh_init ip :
+    messages_history_coh ∅ {[ip := ∅]} {[ip := ∅]}.
+  Proof.
+    rewrite /messages_history_coh
+            /message_soup_coh /receive_buffers_coh /messages_addresses_coh.
+    split; first set_solver.
+    split; first by intros; simplify_map_eq.
+    intros ? ? ? Hgam.
+    split; rewrite get_message_history_empty in Hgam; set_solver.
+  Qed.
+
+  Lemma messages_history_coh_deliver_message mhγ M S Sn Sn' ip sh skt a R m :
+    m ∈ messages_to_receive_at a M →
+    S !! ip = Some Sn →
+    Sn !! sh = Some (skt, R) →
+    Sn' = <[sh:=(skt, R ∪ {[m]})]> Sn →
+    saddress skt = Some a →
+    messages_history_coh M S mhγ →
+    messages_history_coh M (<[ip:=Sn']> S) mhγ.
+  Proof. Admitted.
+
+  Lemma messages_history_drop_message σ mhγ m :
+    messages_history_coh (state_ms σ) (state_sockets σ) mhγ →
+    messages_history_coh (state_ms σ ∖ {[m]}) (state_sockets σ) mhγ.
+  Proof. Admitted.
+
+
+End state_interpretation.
