theories/aneris_lang/state_interp_network_sockets_coh.v
@@ -1,0 +1,490 @@
+From stdpp Require Import fin_maps gmap.
+From iris.bi.lib Require Import fractional.
+From iris.proofmode Require Import tactics.
+From iris.base_logic.lib Require Import viewshifts saved_prop gen_heap.
+From iris_string_ident Require Import ltac2_string_ident.
+From aneris.program_logic Require Export weakestpre adequacy.
+From aneris.program_logic Require Import ectx_lifting.
+From aneris.program_logic Require Export gen_heap_light.
+From aneris.aneris_lang Require Export
+     aneris_lang notation network resources
+     state_interp_def.
+From aneris.aneris_lang.lib Require Import util.
+
+From RecordUpdate Require Import RecordSet.
+Set Default Proof Using "Type".
+
+Import uPred.
+Import Network.
+Import RecordSetNotations.
+
+Section state_interpretation.
+  Context `{!anerisG Σ}.
+
+
+  (** bound_ports_coh *)
+  Lemma bound_ports_coh_alloc_socket Sn P sh skt :
+    Sn !! sh = None →
+    saddress skt = None →
+    bound_ports_coh Sn P →
+    bound_ports_coh (<[sh:=(skt, ∅)]> Sn) P.
+  Proof.
+    intros ??? sh' ???? Hup.
+    destruct (decide (sh = sh')) as [Heq|];
+      simplify_map_eq.
+    - rewrite lookup_insert in Hup. simplify_eq /=.
+      intros. simplify_eq /=.
+    - rewrite lookup_insert_ne in Hup; eauto.
+  Qed.
+
+
+  Lemma bound_ports_coh_socketbind P Sn ps sh skt a :
+    let Sn' := (<[sh:=(skt <| saddress := Some a |>, ∅)]> Sn) in
+    let P' := (<[ip_of_address a:={[port_of_address a]} ∪ ps]> P) in
+    P !! ip_of_address a = Some ps →
+    bound_ports_coh Sn P →
+    bound_ports_coh Sn' P'.
+  Proof.
+    rewrite /bound_ports_coh /=.
+    intros HP HbpsCoh sh' skt' a' P' r' Hsh' Hskt' HP'.
+    destruct (decide (sh' = sh)); simplify_map_eq.
+    - rewrite lookup_insert in Hsh'; simplify_map_eq.
+      rewrite lookup_insert in HP'; by set_solver.
+    - rewrite lookup_insert_ne // in Hsh'.
+      destruct (decide ((ip_of_address a') = (ip_of_address a)))
+        as [Heq|]; simplify_map_eq.
+      + destruct Heq.
+        rewrite lookup_insert in HP'. simplify_eq /=.
+        destruct (decide (port_of_address a' = port_of_address a));
+          [set_solver|].
+        apply elem_of_union_r. by eapply HbpsCoh.
+      + rewrite lookup_insert_ne in HP'; [|done].
+        by eapply HbpsCoh.
+  Qed.
+
+(*
+  Lemma bound_ports_coh_insert_received a skt sh Sn P R T m :
+    Sn !! sh = Some (skt, R, T) →
+    saddress skt = Some a →
+    bound_ports_coh Sn P →
+    bound_ports_coh (<[sh:=(skt, {[m]} ∪ R, T)]> Sn) P.
+  Proof.
+    intros ??? sh' skt' ????.
+    destruct (decide (sh = sh')); simplify_map_eq.
+    - intros; simplify_eq; eauto.
+    - rewrite lookup_insert_ne //; eauto.
+  Qed.
+   *)
+
+  (** socket_handlers_coh *)
+  Lemma socket_handlers_coh_alloc_socket Sn sh s :
+    saddress s = None →
+    socket_handlers_coh Sn →
+    socket_handlers_coh (<[sh:=(s, ∅)]> Sn).
+  Proof.
+    intros ?? sh1 sh2 * ??? H. symmetry in H.
+    ddeq sh1 sh2; ddeq sh1 sh; ddeq sh2 sh; eauto.
+  Qed.
+
+
+  Lemma socket_handlers_coh_socketbind Sn sh skt a :
+    (∀ sh' skt' r' a',
+        Sn !! sh' = Some (skt', r') →
+        saddress skt' = Some a' →
+        port_of_address a' ≠ port_of_address a) →
+    socket_handlers_coh Sn →
+    socket_handlers_coh (<[sh:=(skt <| saddress := Some a |>, ∅)]> Sn).
+  Proof.
+    intros ? Hscoh sh1 sh2 skt1 skt2 ????? Heq.
+    ddeq sh1 sh; ddeq sh2 sh; simplify_eq=>//.
+    - destruct skt, skt2; simplify_map_eq. set_solver.
+    - destruct skt, skt1. simplify_map_eq. set_solver.
+    - destruct skt1, skt2. simplify_map_eq. eapply Hscoh; eauto.
+  Qed.
+
+  (*
+  Lemma socket_handlers_coh_insert_received Sn sh skt m R T :
+    Sn !! sh = Some (skt, R, T) →
+    socket_handlers_coh Sn →
+    socket_handlers_coh (<[sh:=(skt, {[m]} ∪ R, T)]> Sn).
+  Proof.
+    intros ?? sh1 sh2 * ??? H. symmetry in H.
+    ddeq sh1 sh2; ddeq sh1 sh; ddeq sh2 sh; eauto.
+  Qed.
+   *)
+
+  (** socket_messages_coh *)
+  Lemma socket_messages_coh_update_socket Sn sh skt :
+    socket_messages_coh Sn →
+    socket_messages_coh (<[sh:=(skt, ∅)]> Sn).
+  Proof. intros ? sh' **. ddeq sh sh'; [set_solver|]. eauto. Qed.
+
+  Lemma socket_messages_coh_insert_received a sh skt m r Sn :
+    Sn !! sh = Some (skt, r) →
+    m_destination m = a →
+    saddress skt = Some a →
+    socket_messages_coh Sn →
+    socket_messages_coh (<[sh:=(skt, {[m]} ∪ r)]> Sn).
+  Proof.
+    intros ??? Hmcoh sh' skt' r' a' Hsh' ?.
+    destruct (decide (sh = sh')); simplify_eq; last first.
+    { rewrite lookup_insert_ne // in Hsh'. by eapply Hmcoh. }
+    rewrite lookup_insert in Hsh'; simplify_eq.
+    intros m' [?%elem_of_singleton_1 | HR]%elem_of_union; subst; [done|].
+    by eapply Hmcoh.
+  Qed.
+
+  (** socket_addresses_coh *)
+  Lemma socket_addresses_coh_alloc_socket Sn sh skt n :
+    saddress skt = None →
+    socket_addresses_coh Sn n →
+    socket_addresses_coh (<[sh:=(skt, ∅)]> Sn) n.
+  Proof. intros ? ? sh' **. ddeq sh' sh; eauto. Qed.
+
+  Lemma socket_addresses_coh_socketbind Sn sh skt a :
+    saddress skt = None →
+    socket_addresses_coh Sn (ip_of_address a) →
+    socket_addresses_coh (<[sh:=(skt <| saddress := Some a |>, ∅)]> Sn) (ip_of_address a).
+  Proof. intros ? ? sh' **; ddeq sh sh'; eauto. Qed.
+
+  Lemma socket_addresses_coh_insert_received sh a skt m r Sn :
+    saddress skt = Some a →
+    socket_addresses_coh Sn (ip_of_address a) →
+    socket_addresses_coh (<[sh:=(skt, {[m]} ∪ r)]> Sn) (ip_of_address a).
+  Proof. intros ?? sh' **; ddeq sh sh'; eauto. Qed.
+
+  (** socket_unbound_empty_buf_coh *)
+  Lemma socket_unbound_empty_buf_coh_alloc_socket Sn sh ip skt:
+    Sn !! sh = None →
+    saddress skt = None →
+    socket_unbound_empty_buf_coh Sn ip →
+    socket_unbound_empty_buf_coh (<[sh:=(skt, ∅)]> Sn) ip.
+  Proof.
+  Admitted.
+
+  (** network_sockets_coh *)
+  Lemma network_sockets_coh_alloc_node Sn ps ip :
+    Sn !! ip = None →
+    network_sockets_coh Sn ps →
+    network_sockets_coh (<[ip:=∅]> Sn) ps.
+  Proof.
+    rewrite /network_sockets_coh.
+    intros ? Hcoh ip' ? Hst.
+    destruct (decide (ip' = ip)); simplify_eq.
+    - apply lookup_insert_rev in Hst. subst. split; done.
+    - eapply Hcoh; by rewrite lookup_insert_ne in Hst.
+  Qed.
+
+
+    Lemma network_sockets_coh_init n P : network_sockets_coh {[n:= ∅]} P.
+  Proof.
+    rewrite /network_sockets_coh.
+    intros n' Sn' HSn.
+    ddeq n' n;
+      [rewrite lookup_insert in HSn
+      |rewrite lookup_insert_ne in HSn];
+      rewrite /bound_ports_coh
+              /socket_handlers_coh
+              /socket_messages_coh
+              /socket_addresses_coh
+              /socket_unbound_empty_buf_coh;
+      set_solver.
+  Qed.
+
+    Lemma network_sockets_coh_alloc_socket S Sn P n sh skt :
+    S !! n = Some Sn →
+    Sn !! sh = None →
+    saddress skt = None →
+    network_sockets_coh S P →
+    network_sockets_coh (<[n:=<[sh:=(skt, ∅)]> Sn]> S) P.
+  Proof.
+    rewrite /network_sockets_coh.
+    intros ??? Hnets n' Sn' HSn. ddeq n' n; [|eauto].
+    destruct (Hnets n Sn) as (?&?&?&?&?); [done|].
+    split; [by apply bound_ports_coh_alloc_socket|].
+    split; [by apply socket_handlers_coh_alloc_socket|].
+    split; [by apply socket_messages_coh_update_socket|].
+    split; [by apply socket_addresses_coh_alloc_socket |
+            by apply socket_unbound_empty_buf_coh_alloc_socket].
+  Qed.
+
+  Lemma network_sockets_coh_socketbind S P Sn ps sh skt a :
+    let ip := ip_of_address a in
+    let S' := <[ip:= <[sh:= (skt <| saddress := Some a |>, ∅)]> Sn]> S in
+    let P' := (<[ip:={[port_of_address a]} ∪ ps]> P) in
+    S !! ip = Some Sn →
+    P !! ip = Some ps →
+    Sn !! sh = Some (skt, ∅) →
+    port_of_address a ∉ ps →
+    saddress skt = None →
+    network_sockets_coh S P  →
+    network_sockets_coh S' P'.
+  Proof.
+    rewrite /network_sockets_coh /=.
+    intros ????? Hncoh ip Sn' ?.
+    assert
+      (∀ sh' skt' r' a',
+          Sn !! sh' = Some (skt', r') →
+          saddress skt' = Some a' →
+          port_of_address a' ≠ port_of_address a ).
+    { destruct (Hncoh (ip_of_address a) Sn) as
+          (HBpCoh & HshCoh & HmrCoh & HsaCoh);
+        [done|].
+      intros ** Hp.
+      assert (ip_of_address a' = ip_of_address a) as Heq.
+      { eapply HsaCoh; eauto. }
+      assert (port_of_address a' ∈ ps) as Hin.
+      { eapply HBpCoh; eauto. rewrite Heq //. }
+      rewrite Hp in Hin. set_solver. }
+    ddeq ip (ip_of_address a).
+    - destruct (Hncoh (ip_of_address a) Sn) as (?&?&?&?&?); [done|].
+      split; [by eapply bound_ports_coh_socketbind|].
+      split; [by eapply socket_handlers_coh_socketbind|].
+      split; [by eapply socket_messages_coh_update_socket|].
+      split; [by eapply socket_addresses_coh_socketbind |].
+      admit.
+    - destruct (Hncoh ip Sn') as (HBpCoh & HshCoh & HmrCoh & HsaCoh); [done|].
+      split; [|done].
+      intros ? skt' a' ???? Hps.
+      assert (ip_of_address a' = ip).
+      { eapply HsaCoh; eauto. }
+      simplify_eq /=. rewrite lookup_insert_ne in Hps; [|done].
+      by eapply HBpCoh.
+  Admitted.
+
+
+  Lemma network_sockets_coh_deliver_message M P S Sn Sn' ip sh skt a R m :
+    m ∈ messages_to_receive_at a M →
+    S !! ip = Some Sn →
+    Sn !! sh = Some (skt, R) →
+    Sn' = <[sh:=(skt, R ∪ {[m]})]> Sn →
+    saddress skt = Some a →
+    network_sockets_coh S P →
+    network_sockets_coh (<[ip:=Sn']> S) P.
+  Proof. Admitted.
+
+  (*
+  Lemma network_sockets_coh_insert_sent S P M Sn sh skt a to m R T :
+    let ip := ip_of_address a in
+    let msg := mkMessage a to (sprotocol skt) m in
+    saddress skt = Some a →
+    S !! ip = Some Sn →
+    Sn !! sh = Some (skt, R, T) →
+    network_sockets_coh S M P →
+    network_sockets_coh (<[ip:=<[sh:=(skt, R, {[msg]} ∪ T)]> Sn]> S) ({[msg]} ∪ M) P.
+  Proof.
+    intros ip msg Hsa Hsi Hh HnetCoh ip' Sn' Hip'.
+    ddeq ip' ip.
+    - destruct (HnetCoh ip Sn Hsi) as (HBpCoh & HshCoh & HsmCoh & HsaCoh).
+      split.
+      { intros sh' skt' **. ddeq sh' sh; eauto using HBpCoh. }
+      split.
+      { intros sh1 sh2 skt1 skt2 ???? Hsh1 Hsh2 Hskt1 Hsaddr.
+        ddeq sh1 sh; ddeq sh2 sh; simplify_eq /=;
+          eapply HshCoh; eauto; eapply mk_is_Some; rewrite Hsaddr //. }
+      split.
+      { intros sh' **; ddeq sh' sh; split; intros;
+          edestruct HsmCoh; set_solver. }
+      intros sh' **; ddeq sh' sh; eauto.
+    - destruct (HnetCoh ip' Sn' Hip') as (HBpCoh & HshCoh & HsmCoh & HsaCoh).
+      split; eauto. split; eauto. split; last done.
+      intros sh' **. edestruct HsmCoh; eauto.
+      split; intros ??; set_solver.
+  Qed.
+
+  Lemma network_sockets_coh_not_received a skt sh S Sn P M R T m :
+    S !! ip_of_address a = Some Sn →
+    Sn !! sh = Some (skt, R, T) →
+    saddress skt = Some a →
+    m_destination m = a →
+    m ∈ M →
+    m ∉ R →
+    network_sockets_coh S M P →
+    ¬ message_received S m.
+  Proof.
+    intros HS HSn Hskt Hd HM HR Hsock Hr.
+    destruct Hr as (Sn' & sh' & skt' & a' & R' & T' & HS' & HSn' & Hs' & Hm).
+    destruct (decide (a = a')) as [ | Ha]; simplify_eq.
+    - assert (sh = sh') as <-.
+      { eapply Hsock; eauto. rewrite Hs' //. }
+      by simplify_eq.
+    - destruct (Hsock (ip_of_address a') Sn')
+        as (?&Hhandlers'&Hmsg'&?); [done|].
+      destruct (Hmsg' _ _ _ _ a' HSn') as [HR' ?]; [done|].
+      by destruct (HR' _ Hm) as [? ?].
+  Qed.
+
+  Lemma network_sockets_coh_insert_received a skt sh S Sn P M R T m :
+    let S' := (<[ip_of_address a:=<[sh:=(skt, {[m]} ∪ R, T)]> Sn]> S) in
+    S !! ip_of_address a = Some Sn →
+    Sn !! sh = Some (skt, R, T) →
+    saddress skt = Some a →
+    m_destination m = a →
+    m ∈ M →
+    m ∉ R →
+    network_sockets_coh S M P →
+    network_sockets_coh S' M P.
+  Proof.
+    rewrite /network_sockets_coh.
+    intros HS HSn ???? Hnet ip' Sn' HSn'.
+    destruct (decide (ip_of_address a = ip'));
+      simplify_map_eq; [|by eapply Hnet].
+    destruct (Hnet _ _ HS) as (?&?&?&?).
+    split; [by eapply bound_ports_coh_insert_received|].
+    split; [by eapply socket_handlers_coh_insert_received|].
+    split; [by eapply socket_messages_coh_insert_received|].
+    by eapply socket_addresses_coh_insert_received.
+  Qed.
+
+  Lemma network_sockets_messages_coh_insert_received a skt sh S Sn P M R T m :
+    let S' := (<[ip_of_address a:=<[sh:=(skt, {[m]} ∪ R, T)]> Sn]> S) in
+    S !! ip_of_address a = Some Sn →
+    Sn !! sh = Some (skt, R, T) →
+    saddress skt = Some a →
+    m_destination m = a →
+    m ∈ M →
+    m ∉ R →
+    network_sockets_coh S M P →
+    network_messages_coh S M -∗
+    network_messages_coh S' M ∗
+      ∃ φ : socket_interp Σ, m_destination m ⤇ φ ∗ ▷ φ m.
+  Proof.
+    iIntros (S' ???????) "Hmcoh".
+    rewrite /network_messages_coh big_sepS_delete //.
+    iDestruct "Hmcoh" as "[[Hm | %Hr] Hmsgs]";
+      [|exfalso; by eapply network_sockets_coh_not_received].
+    iFrame.
+    assert (message_received S' m) as Hr.
+    { by eapply message_received_receive. }
+    rewrite (big_sepS_delete _ M m) //. iFrame "%".
+    iApply big_sepS_mono; [|done].
+    iIntros (??) "[? | %Hr']"; [eauto|].
+    iRight. iPureIntro.
+    by eapply message_received_insert.
+  Qed.
+*)
+
+  (*
+  (** network_coh **)
+  Lemma network_coh_init ip ips P :
+    dom (gset ip_address) P = ips →
+    (∀ ip, ip ∈ ips → P !! ip = Some ∅) →
+    ⊢ network_sockets_coh {[ip:=∅]} ∅ P.
+  Proof.
+    intros ??. rewrite /network_coh /network_messages_coh.
+    iSplit; [|done].
+    iPureIntro. rewrite /network_sockets_coh.
+    intros ?? [<- <-]%lookup_singleton_Some.
+    rewrite /bound_ports_coh /socket_handlers_coh
+            /socket_messages_coh /socket_addresses_coh.
+    set_solver.
+  Qed.
+
+   *)
+
+  (*
+  Lemma network_coh_sent_valid m sh a skt S Sn M P R T :
+    S !! ip_of_address a = Some Sn →
+    Sn !! sh = Some (skt, R, T) →
+    saddress skt = Some a →
+    m ∈ T →
+    network_coh S M P -∗ ⌜m ∈ M⌝.
+  Proof.
+    iIntros (Hs HSn Ha Hm) "(%Hscoh & _)". iPureIntro.
+    destruct (Hscoh _ Sn Hs) as (?&?& Hmsgs &?).
+    edestruct (Hmsgs sh) as [? HT]; [done..|].
+    by apply HT.
+  Qed.
+
+  Lemma network_coh_received_valid m sh a skt S Sn M P R T :
+    S !! ip_of_address a = Some Sn →
+    Sn !! sh = Some (skt, R, T) →
+    saddress skt = Some a →
+    m ∈ R →
+    network_coh S M P -∗ ⌜m ∈ M⌝.
+  Proof.
+    iIntros (Hs HSn Ha Hm) "(%Hscoh & _)". iPureIntro.
+    destruct (Hscoh _ Sn Hs) as (?&?& Hmsgs &?).
+    edestruct (Hmsgs sh) as [HR ?]; [done..|].
+    by apply HR.
+  Qed.
+
+  Lemma network_coh_alloc_node Sn M ps ip :
+    Sn !! ip = None →
+    network_coh Sn M ps -∗
+    network_coh (<[ip:=∅]>Sn) M ps.
+  Proof.
+    iIntros (Hnone) "[% Hmsg]".
+    rewrite /network_coh.
+    iSplitR; last first.
+    { by iApply network_messages_coh_alloc_node. }
+    iPureIntro.
+    by apply network_sockets_coh_alloc_node.
+  Qed.
+
+  Lemma network_coh_alloc_socket S M P Sn n sh skt :
+    S !! n = Some Sn →
+    Sn !! sh = None →
+    saddress skt = None →
+    network_coh S M P -∗
+    network_coh (<[n:=<[sh:=(skt, ∅, ∅)]> Sn]> S) M P.
+  Proof.
+    iIntros (? ? ?) "(% & Hmsg)". iSplitR.
+    - iPureIntro. by apply network_sockets_coh_alloc_socket.
+    - by iApply network_messages_coh_alloc_socket.
+  Qed.
+
+  Lemma network_coh_socketbind S P M Sn ps sh skt a :
+    let ip := ip_of_address a in
+    S !! ip = Some Sn →
+    Sn !! sh = Some (skt, ∅, ∅) →
+    P !! ip = Some ps →
+    saddress skt = None →
+    port_of_address a ∉ ps →
+    network_coh S M P -∗
+    network_coh
+    (<[ip:=<[sh:=(skt <| saddress := Some a |>, ∅, ∅)]> Sn]> S) M
+    (<[ip:= {[port_of_address a]} ∪ ps]> P).
+  Proof.
+    iIntros (??????) "(% & Hmsg)". iSplit.
+    - iPureIntro; by apply network_sockets_coh_socketbind.
+    - by iDestruct (network_messages_coh_socketbind with "Hmsg") as "Hmsg".
+  Qed.
+
+  Lemma network_coh_insert_sent S P M Sn sh skt a to m (φ : socket_interp Σ) R T :
+    let ip := ip_of_address a in
+    let msg := mkMessage a to (sprotocol skt) m in
+    let S' := <[ip := <[sh:=(skt, R, {[msg]} ∪ T)]> Sn]> S in
+    let M' := {[msg]} ∪ M in
+    saddress skt = Some a →
+    S !! ip = Some Sn →
+    Sn !! sh = Some (skt, R, T) →
+    to ⤇ φ -∗
+    φ msg -∗
+    network_coh S M P -∗ network_coh S' M' P.
+  Proof.
+    iIntros (???????) "Hpred Hr [% Hmsg]". iSplit.
+    - iPureIntro. by apply network_sockets_coh_insert_sent.
+    - by iApply (network_messages_coh_insert_sent with "Hpred Hr Hmsg").
+  Qed.
+
+  Lemma network_coh_receive a sh skt S Sn M P R T m :
+    let ip := ip_of_address a in
+    let S' := (<[ip:=<[sh:=(skt, {[m]} ∪ R, T)]> Sn]> S) in
+    saddress skt = Some a →
+    S !! ip = Some Sn →
+    Sn !! sh = Some (skt, R, T) →
+    m_destination m = a →
+    m ∈ M →
+    m ∉ R →
+    network_coh S M P -∗ network_coh S' M P ∗ ∃ φ, m_destination m ⤇ φ ∗ ▷ φ m.
+  Proof.
+    simpl. iIntros (??????) "[%Hsock Hmcoh]".
+    rewrite /network_coh.
+    iDestruct (network_sockets_messages_coh_insert_received with "Hmcoh")
+      as "[Hmcoh Hφ]"; [done..|].
+    iFrame. iPureIntro.
+    by apply network_sockets_coh_insert_received.
+   Qed.*)
+
+End state_interpretation.
