theories/aneris_lang/state_interp_socket_interp_coh.v
@@ -1,0 +1,153 @@
+From stdpp Require Import fin_maps gmap.
+From iris.bi.lib Require Import fractional.
+From iris.proofmode Require Import tactics.
+From iris.base_logic.lib Require Import viewshifts saved_prop gen_heap.
+From iris_string_ident Require Import ltac2_string_ident.
+From aneris.program_logic Require Export weakestpre adequacy.
+From aneris.program_logic Require Import ectx_lifting.
+From aneris.program_logic Require Export gen_heap_light.
+From aneris.aneris_lang Require Export
+     aneris_lang notation network resources
+     state_interp_def.
+From aneris.aneris_lang.lib Require Import util.
+
+From RecordUpdate Require Import RecordSet.
+Set Default Proof Using "Type".
+
+Import uPred.
+Import Network.
+Import RecordSetNotations.
+
+Section state_interpretation.
+  Context `{!anerisG Σ}.
+
+  (** socket_interp_coh *)
+  Lemma socket_interp_coh_init ips A M σ f :
+    dom (gset _) M = A →
+    dom (gset _) (state_ports_in_use σ) = ips →
+    (∀ ip, ip ∈ ips → state_ports_in_use σ !! ip = Some ∅) →
+    (∀ a, a ∈ A → ip_of_address a ∈ ips) →
+    ([∗ set] a ∈ A, a ⤇ f a)%I -∗
+    fixed A -∗
+    saved_si_auth M -∗
+    socket_interp_coh (state_ports_in_use σ).
+  Proof.
+    iIntros (Hdmsi Hipdom Hpiiu Hfixdom) "? ? ?".
+    rewrite /socket_interp_coh. iExists _; iFrame.
+    iExists _; iFrame; iFrame "#".
+    rewrite -!Hdmsi.
+    iSplit; [iApply (big_sepS_mono with "[$]"); auto|].
+    iSplit; [iPureIntro; set_solver|].
+    iPureIntro. intros b Hbips. split; auto.
+    intros [Hb | [Hb HP]]; [done|].
+    simplify_eq.
+    specialize (Hpiiu _ Hbips).
+    specialize (HP _ Hpiiu). done.
+  Qed.
+
+  Lemma socket_interp_coh_fixed_valid a A ips :
+    a ∈ A →
+    socket_interp_coh ips -∗ fixed A -∗ ∃ φ, a ⤇ φ.
+  Proof.
+    iIntros (HaA) "Hscoh #HA".
+    iDestruct "Hscoh" as (si A') "(HA' & Hsiauth & Hsis & % & H)".
+    iDestruct "H" as %Hdom.
+    iDestruct (fixed_agree with "HA HA'") as %->.
+    iDestruct (big_sepS_elem_of with "Hsis") as "$".
+    erewrite Hdom; eauto.
+  Qed.
+
+  Lemma socket_interp_coh_socketbind_static ps P a A:
+    a ∈ A →
+    P !! ip_of_address a = Some ps →
+    port_of_address a ∉ ps →
+    fixed A -∗
+    socket_interp_coh P -∗
+    socket_interp_coh (<[ip_of_address a:={[port_of_address a]} ∪ ps]> P).
+  Proof.
+    iIntros (???) "HA". rewrite /socket_interp_coh.
+    iDestruct 1 as (si A') "(HA' & Hsiauth & Hsis & %Hf & %Hdms)".
+    iDestruct (fixed_agree with "HA HA'") as %->.
+    iExists _,_. iFrame. iPureIntro. split.
+    { intros ??. rewrite dom_insert elem_of_union; right. by apply Hf. }
+    intros b. rewrite dom_insert elem_of_union. intros Hb.
+    rewrite Hdms; last first.
+    { destruct (decide (a = b)); subst; first by apply Hf.
+      destruct Hb as [->%elem_of_singleton_1|]; [|done]. by apply Hf. }
+    split; intros [|[Hnb Hdm]]; auto.
+    { right. split; [done|].
+      destruct (decide (ip_of_address a = ip_of_address b)) as [Heq|].
+      - intros P'. rewrite Heq lookup_insert. intros; simplify_eq.
+        apply elem_of_union_r, Hdm. rewrite -Heq //.
+      - intros P'. rewrite lookup_insert_ne //. apply Hdm. }
+    destruct (decide (ip_of_address a = ip_of_address b)) as [Heq|].
+    { right. split; [done|]. intros P'.
+      rewrite Heq lookup_insert in Hdm.
+      specialize (Hdm ({[port_of_address a]} ∪ _) eq_refl).
+      apply elem_of_union in Hdm. destruct Hdm as [Hdm%elem_of_singleton_1 | Hdm].
+      - destruct a, b; simpl in *. by subst.
+      - rewrite -Heq. by intros; simplify_eq. }
+    right. split; [done|].
+    rewrite lookup_insert_ne in Hdm; done.
+  Qed.
+
+  Lemma socket_interp_coh_socketbind_dynamic ps P a A φ :
+    a ∉ A →
+    P !! ip_of_address a = Some ps →
+    port_of_address a ∉ ps →
+    fixed A -∗
+    socket_interp_coh P ==∗
+    socket_interp_coh (<[ip_of_address a:={[port_of_address a]} ∪ ps]> P) ∗
+    a ⤇ φ.
+  Proof.
+    iIntros (? Hpa Hps) "#HA". rewrite /socket_interp_coh.
+    iDestruct 1 as (si A') "(HA' & Hsiauth & Hsis & %Hf & %Hdms)".
+    iDestruct (fixed_agree with "HA HA'") as %<-.
+    assert (si !! a = None).
+    { destruct (si !! a) eqn:Heq; last done.
+      destruct (Hdms a) as [[|[Hfx HP]] _]; try done.
+      - by eapply elem_of_dom_2.
+      - rewrite elem_of_dom. eauto.
+      - by apply HP in Hpa. }
+    iMod (socket_interp_alloc a φ with "Hsiauth")
+      as (?) "[Hsiauth #Hφ]"; [done|].
+    iFrame "Hφ". iModIntro. iExists _, _; iFrame.
+    iSplitL "Hsis".
+    { rewrite dom_insert_L big_sepS_insert;
+        last rewrite not_elem_of_dom //.
+      iFrame. iExists _. iFrame "Hφ". }
+    iSplit.
+    { iPureIntro. intros b Hb.
+      destruct (decide (a = b)); subst; first done.
+      apply dom_insert, elem_of_union. by auto. }
+    iPureIntro. intros b Hbdom.
+    rewrite dom_insert elem_of_union elem_of_singleton Hdms; last first.
+    { destruct (decide (ip_of_address a = ip_of_address b)) as [Heq|].
+      - destruct Heq. by eapply elem_of_dom_2.
+      - apply dom_insert, elem_of_union in Hbdom. set_solver. }
+    split.
+    - intros [Hb | Hdom]; subst.
+      + right. split; [done|]. rewrite lookup_insert.
+        intros; simplify_eq. by apply elem_of_union_l, elem_of_singleton.
+      + destruct Hdom as [? | [Hb HP]]; first by left.
+        right. split; first done.
+        destruct (decide (ip_of_address a = ip_of_address b)) as [Heq |Hneq].
+        * destruct Heq. rewrite lookup_insert. intros; simplify_eq.
+          apply elem_of_union_r, HP; eauto.
+        * by rewrite lookup_insert_ne.
+    - intros [Hb | [Hb Hdom]]; first by auto.
+      destruct (decide (a = b)) as [Heq | Hneq]; first by auto.
+      right; right. split; first done.
+      destruct (decide (ip_of_address a = ip_of_address b)) as [Heq|].
+      + intros ps'.
+        rewrite Heq in Hdom.
+        rewrite lookup_insert in Hdom.
+        specialize (Hdom ({[port_of_address a]} ∪ ps) eq_refl).
+        apply elem_of_union in Hdom. destruct Hdom as [Hdom | Hport].
+        * apply elem_of_singleton_1 in Hdom.
+          destruct a,b; simpl in *; simplify_eq.
+        * intros. destruct Heq; simplify_eq; eauto.
+      + intros. apply Hdom. rewrite lookup_insert_ne //.
+  Qed.
+
+End state_interpretation.
